proof/agp32_ID_CorrectScript.sml
@@ -681,13 +681,76 @@ Proof
 QED
 
 
+(** lemmas for ID_read_dataA/B/W **)
+(** when ID stage is disabled, some items are the same as before **)
+(** ID_addrA/B/W **)
+Theorem agp32_ID_disabled_ID_addr_unchanged[local]:
+  !fext fbits a t I.
+    is_sch_decode I (agp32 fext fbits) a ==>
+    is_sch_disable I (agp32 fext fbits) ==>
+    Rel I (fext t) (agp32 fext fbits (t-1)) (agp32 fext fbits t) a t ==>
+    I (2,SUC t) <> NONE ==>
+    ~enable_stg 2 (agp32 fext fbits t) ==>
+    ((agp32 fext fbits (SUC t)).ID.ID_addrA = (agp32 fext fbits t).ID.ID_addrA) /\
+    ((agp32 fext fbits (SUC t)).ID.ID_addrB = (agp32 fext fbits t).ID.ID_addrB) /\
+    ((agp32 fext fbits (SUC t)).ID.ID_addrW = (agp32 fext fbits t).ID.ID_addrW)
+Proof
+  rpt gen_tac >> rpt disch_tac >>
+  `((agp32 fext fbits (SUC t)).ID.ID_addrA = addrA (FUNPOW Next (THE (I' (2,SUC t)) − 1) a)) /\
+  ((agp32 fext fbits (SUC t)).ID.ID_addrB = addrB (FUNPOW Next (THE (I' (2,SUC t)) − 1) a)) /\
+  ((agp32 fext fbits (SUC t)).ID.ID_addrW = addrW (FUNPOW Next (THE (I' (2,SUC t)) − 1) a))`
+    by fs [agp32_Rel_ag32_ID_addr_correct] >>
+  `I' (2,SUC t) = I' (2,t)` by fs [is_sch_disable_def] >>
+  fs [Rel_def,ID_Rel_def]
+QED
+
+(** ID_addrA/B/W_disable **)
+Theorem agp32_ID_disabled_ID_flag_unchanged[local]:
+  !fext fbits a t I.
+    is_sch_decode I (agp32 fext fbits) a ==>
+    is_sch_disable I (agp32 fext fbits) ==>
+    Rel I (fext t) (agp32 fext fbits (t-1)) (agp32 fext fbits t) a t ==>
+    I (2,SUC t) <> NONE ==>
+    ~enable_stg 2 (agp32 fext fbits t) ==>
+    ((agp32 fext fbits (SUC t)).ID.ID_addrA_disable = (agp32 fext fbits t).ID.ID_addrA_disable) /\
+    ((agp32 fext fbits (SUC t)).ID.ID_addrB_disable = (agp32 fext fbits t).ID.ID_addrB_disable) /\
+    ((agp32 fext fbits (SUC t)).ID.ID_addrW_disable = (agp32 fext fbits t).ID.ID_addrW_disable)
+Proof
+  rpt gen_tac >> rpt disch_tac >>
+  `((agp32 fext fbits (SUC t)).ID.ID_addrA_disable = flagA (FUNPOW Next (THE (I' (2,SUC t)) − 1) a)) /\
+  ((agp32 fext fbits (SUC t)).ID.ID_addrB_disable = flagB (FUNPOW Next (THE (I' (2,SUC t)) − 1) a)) /\
+  ((agp32 fext fbits (SUC t)).ID.ID_addrW_disable = flagW (FUNPOW Next (THE (I' (2,SUC t)) − 1) a))`
+    by fs [agp32_Rel_ag32_ID_flag_correct] >>
+  `I' (2,SUC t) = I' (2,t)` by fs [is_sch_disable_def] >>
+  fs [Rel_def,ID_Rel_def]
+QED
+
+(** ID_read_dataA/B/W **)
+Theorem agp32_ID_disabled_ID_read_data_unchanged[local]:
+  !fext fbits a t I.
+    is_sch_decode I (agp32 fext fbits) a ==>
+    is_sch_disable I (agp32 fext fbits) ==>
+    Rel I (fext t) (agp32 fext fbits (t-1)) (agp32 fext fbits t) a t ==>
+    I (2,SUC t) <> NONE ==>
+    ~enable_stg 2 (agp32 fext fbits t) ==>
+    ~enable_stg 5 (agp32 fext fbits t) ==>
+    ((agp32 fext fbits (SUC t)).ID.ID_read_dataA = (agp32 fext fbits t).ID.ID_read_dataA) /\
+    ((agp32 fext fbits (SUC t)).ID.ID_read_dataB = (agp32 fext fbits t).ID.ID_read_dataB) /\
+    ((agp32 fext fbits (SUC t)).ID.ID_read_dataW = (agp32 fext fbits t).ID.ID_read_dataW)
+Proof
+  rpt gen_tac >> rpt disch_tac >>
+  fs [agp32_ID_read_data_rewrite_R_and_ID_addr] >>
+  METIS_TAC [agp32_WB_disabled_then_R_unchanged,agp32_ID_disabled_ID_addr_unchanged]
+QED
+
+
 (** ID_read_dataA: when instrs in EX, MEM and WB do not change registers **)
 Theorem agp32_Rel_ag32_ID_read_dataA_no_write_before:
   !fext fbits a t I.
     is_sch I (agp32 fext fbits) a ==>
     Rel I (fext t) (agp32 fext fbits (t-1)) (agp32 fext fbits t) a t ==>
-    enable_stg 2 (agp32 fext fbits t) ==>
     I (2,SUC t) <> NONE ==>
+    ~(agp32 fext fbits (SUC t)).ID.ID_addrA_disable ==>
     ~reg_adr_update_isa (I (3,SUC t)) a (agp32 fext fbits (SUC t)).ID.ID_addrA ==>
     ~reg_adr_update_isa (I (4,SUC t)) a (agp32 fext fbits (SUC t)).ID.ID_addrA ==>
     ~reg_adr_update_isa (I (5,SUC t)) a (agp32 fext fbits (SUC t)).ID.ID_addrA ==>
@@ -814,121 +877,336 @@ Proof
     `THE (I' (4,SUC t)) = THE (I' (3,SUC t)) - 1` by FULL_SIMP_TAC std_ss [] >>
     METIS_TAC [reg_adr_update_isa_not_change_data]) >-
    (** I (5,t) is not NONE **)
-   (`s.WB.WB_state_flag` by fs [Abbr `s`,enable_stg_def,agp32_ID_ID_write_enable_WB_state_flag] >>
-    `wb_data_vaild s` by fs [Abbr `s`,wb_data_vaild_def] >>
-    `(agp32 fext fbits (SUC t)).R = (FUNPOW Next (THE (I' (5,t))) a).R` by cheat >> fs [] >>
-    subgoal `I' (2,SUC t) = I' (1,t)` >-
-     (fs [is_sch_def,is_sch_decode_def,Abbr `s`] >>
-      METIS_TAC []) >> fs [] >>
-    subgoal `I' (5,SUC t) = I' (4,t)` >-
-     (fs [is_sch_def,is_sch_writeback_def,is_sch_disable_def,Abbr `s`] >>
-      Cases_on `enable_stg 5 (agp32 fext fbits t)` >>
-      METIS_TAC []) >> fs [] >>
-    subgoal `I' (4,SUC t) = I' (3,t)` >-
-     (fs [is_sch_def,is_sch_memory_def,Abbr `s`] >>
-      `enable_stg 4 (agp32 fext fbits t)`
-        by fs [enable_stg_def,agp32_ID_ID_write_enable_MEM_state_flag] >>
-      Cases_on `isMemOp_hw_op (agp32 fext fbits t)` >>
-      fs [enable_stg_def] >>
-      METIS_TAC [MEM_stg_op_agp32_ID_EX_write_disable,
-                 agp32_ID_ID_write_enable_and_ID_EX_write_enable]) >> fs [] >>
-    subgoal `I' (3,SUC t) = I' (2,t)` >-
-     (fs [is_sch_def,is_sch_execute_def,Abbr `s`] >>
-      `enable_stg 3 (agp32 fext fbits t)`
-        by fs [enable_stg_def,agp32_ID_ID_write_enable_and_ID_EX_write_enable] >>
-      Cases_on `isJump_hw_op (agp32 fext fbits t)` >-
-       (`isJump_isa_op (I' (3,t)) a` by fs [isJump_hw_op_def,Rel_def,EX_Rel_spec_def] >>
-         METIS_TAC [isJump_isa_op_not_none]) >>
-      Cases_on `~reg_data_hazard (agp32 fext fbits t)` >- METIS_TAC [] >>
-      fs [isJump_hw_op_def,enable_stg_def] >>
-      METIS_TAC [agp32_ID_ID_write_enable_EX_jump_sel_then_no_reg_data_hazard]) >> fs [] >>
-    `THE (I' (1,t)) = THE (I' (5,t)) + 1`
-      by METIS_TAC [ID_EX_MEM_NONE_IF_instr_index_with_WB_instr_plus_1] >> fs []) >-
+   (Cases_on `s.WB.WB_state_flag` >-
+     (`wb_data_vaild s` by fs [Abbr `s`,wb_data_vaild_def] >>
+      `(agp32 fext fbits (SUC t)).R = (FUNPOW Next (THE (I' (5,t))) a).R` by cheat >> fs [] >>
+      Cases_on `enable_stg 2 (agp32 fext fbits t)` >-
+       (subgoal `I' (2,SUC t) = I' (1,t)` >-
+         (fs [is_sch_def,is_sch_decode_def,Abbr `s`] >>
+          METIS_TAC []) >> fs [] >>
+        subgoal `I' (5,SUC t) = I' (4,t)` >-
+         (fs [is_sch_def,is_sch_writeback_def,is_sch_disable_def,Abbr `s`] >>
+          Cases_on `enable_stg 5 (agp32 fext fbits t)` >>
+          METIS_TAC []) >> fs [] >>
+        subgoal `I' (4,SUC t) = I' (3,t)` >-
+         (fs [is_sch_def,is_sch_memory_def,Abbr `s`] >>
+          `enable_stg 4 (agp32 fext fbits t)`
+            by fs [enable_stg_def,agp32_ID_ID_write_enable_MEM_state_flag] >>
+          Cases_on `isMemOp_hw_op (agp32 fext fbits t)` >>
+          fs [enable_stg_def] >>
+          METIS_TAC [MEM_stg_op_agp32_ID_EX_write_disable,
+                     agp32_ID_ID_write_enable_and_ID_EX_write_enable]) >> fs [] >>
+        subgoal `I' (3,SUC t) = I' (2,t)` >-
+         (fs [is_sch_def,is_sch_execute_def,Abbr `s`] >>
+          `enable_stg 3 (agp32 fext fbits t)`
+            by fs [enable_stg_def,agp32_ID_ID_write_enable_and_ID_EX_write_enable] >>
+          Cases_on `isJump_hw_op (agp32 fext fbits t)` >-
+           (`isJump_isa_op (I' (3,t)) a` by fs [isJump_hw_op_def,Rel_def,EX_Rel_spec_def] >>
+            METIS_TAC [isJump_isa_op_not_none]) >>
+          Cases_on `~reg_data_hazard (agp32 fext fbits t)` >- METIS_TAC [] >>
+          fs [isJump_hw_op_def,enable_stg_def] >>
+          METIS_TAC [agp32_ID_ID_write_enable_EX_jump_sel_then_no_reg_data_hazard]) >> fs [] >>
+        `THE (I' (1,t)) = THE (I' (5,t)) + 1`
+          by METIS_TAC [ID_EX_MEM_NONE_IF_instr_index_with_WB_instr_plus_1] >> fs []) >>
+      `I' (2,SUC t) = I' (2,t)` by fs [is_sch_def,is_sch_disable_def] >>
+      subgoal `I' (5,SUC t) = I' (4,t)` >-
+       (fs [is_sch_def,is_sch_writeback_def,is_sch_disable_def,Abbr `s`] >>
+        Cases_on `enable_stg 5 (agp32 fext fbits t)` >>
+        METIS_TAC []) >> fs [] >>
+      Cases_on `enable_stg 3 (agp32 fext fbits t)` >-
+       (subgoal `I' (4,SUC t) = I' (3,t)` >-
+         (fs [is_sch_def,is_sch_memory_def,Abbr `s`] >>
+          `enable_stg 4 (agp32 fext fbits t)`
+            by fs [enable_stg_def,agp32_MEM_state_flag_eq_WB_state_flag] >>
+          Cases_on `isMemOp_hw_op (agp32 fext fbits t)` >>
+          fs [enable_stg_def] >>
+          METIS_TAC [MEM_stg_op_agp32_ID_EX_write_disable,enable_stg_def]) >> fs [] >>
+        `THE (I' (2,t)) = THE (I' (5,t)) + 1`
+          by METIS_TAC [EX_MEM_NONE_ID_instr_index_with_WB_instr_plus_1] >> fs []) >>
+      `I' (3,SUC t) = I' (3,t)` by METIS_TAC [is_sch_def,is_sch_disable_def] >>
+      `THE (I' (2,t)) = THE (I' (5,t)) + 1`
+        by METIS_TAC [EX_MEM_NONE_ID_instr_index_with_WB_instr_plus_1] >> fs []) >>
+    `~enable_stg 5 (agp32 fext fbits t)` by fs [enable_stg_def] >>
+    `I' (5,SUC t) = I' (5,t)` by METIS_TAC [is_sch_def,is_sch_disable_def] >> fs []) >-
    (** I (3,SUC t) and I (5,t) are not NONE **)
-   (`s.WB.WB_state_flag` by fs [Abbr `s`,enable_stg_def,agp32_ID_ID_write_enable_WB_state_flag] >>
-    `wb_data_vaild s` by fs [Abbr `s`,wb_data_vaild_def] >>
-    `(agp32 fext fbits (SUC t)).R = (FUNPOW Next (THE (I' (5,t))) a).R` by cheat >> fs [] >>
-    `(agp32 fext fbits (SUC t)).ID.ID_addrA = (22 >< 17) i`
-      by (fs [Abbr `i`,Abbr `s`,is_sch_def] >>
-          METIS_TAC [agp32_Rel_ag32_ID_addr_correct,addrA_def]) >> fs [] >>
-    subgoal `I' (2,SUC t) = I' (1,t)` >-
-     (fs [is_sch_def,is_sch_decode_def,Abbr `s`] >>
-      METIS_TAC []) >> fs [] >>
-    subgoal `I' (5,SUC t) = I' (4,t)` >-
-     (fs [is_sch_def,is_sch_writeback_def,is_sch_disable_def,Abbr `s`] >>
-      Cases_on `enable_stg 5 (agp32 fext fbits t)` >>
-      METIS_TAC []) >> fs [] >>
-    subgoal `I' (4,SUC t) = I' (3,t)` >-
-     (fs [is_sch_def,is_sch_memory_def,Abbr `s`] >>
-      `enable_stg 4 (agp32 fext fbits t)`
-        by fs [enable_stg_def,agp32_ID_ID_write_enable_MEM_state_flag] >>
-      Cases_on `isMemOp_hw_op (agp32 fext fbits t)` >>
-      fs [enable_stg_def] >>
-      METIS_TAC [MEM_stg_op_agp32_ID_EX_write_disable,
-                 agp32_ID_ID_write_enable_and_ID_EX_write_enable]) >> fs [] >>
-    subgoal `I' (3,SUC t) = I' (2,t)` >-
-     (fs [is_sch_def,is_sch_execute_def,Abbr `s`] >>
-      `enable_stg 3 (agp32 fext fbits t)`
-        by fs [enable_stg_def,agp32_ID_ID_write_enable_and_ID_EX_write_enable] >>
-      Cases_on `isJump_isa_op (I' (3,t)) a` >-
-       METIS_TAC [isJump_isa_op_not_none] >>
-      Cases_on `~reg_data_hazard (agp32 fext fbits t)` >>
-      METIS_TAC []) >> fs [] >>
-    `THE (I' (2,t)) = THE (I' (5,t)) + 1`
-      by METIS_TAC [EX_MEM_NONE_ID_instr_index_with_WB_instr_plus_1] >>
-    `THE (I' (5,t)) = THE (I' (2,t)) - 1` by fs [] >>
-    `THE (I' (1,t)) = THE (I' (2,t)) + 1`
-      by METIS_TAC [IF_instr_index_with_ID_instr_plus_1] >> fs [] >>
-    METIS_TAC [reg_adr_update_isa_not_change_data]) >-
+   (Cases_on `s.WB.WB_state_flag` >-
+     (`wb_data_vaild s` by fs [Abbr `s`,wb_data_vaild_def] >>
+      `(agp32 fext fbits (SUC t)).R = (FUNPOW Next (THE (I' (5,t))) a).R` by cheat >> fs [] >>
+      `(agp32 fext fbits (SUC t)).ID.ID_addrA = (22 >< 17) i`
+        by (fs [Abbr `i`,Abbr `s`,is_sch_def] >>
+            METIS_TAC [agp32_Rel_ag32_ID_addr_correct,addrA_def]) >> fs [] >>
+       Cases_on `enable_stg 2 (agp32 fext fbits t)` >-
+       (subgoal `I' (2,SUC t) = I' (1,t)` >-
+         (fs [is_sch_def,is_sch_decode_def,Abbr `s`] >>
+          METIS_TAC []) >> fs [] >>
+        subgoal `I' (5,SUC t) = I' (4,t)` >-
+         (fs [is_sch_def,is_sch_writeback_def,is_sch_disable_def,Abbr `s`] >>
+          Cases_on `enable_stg 5 (agp32 fext fbits t)` >>
+          METIS_TAC []) >> fs [] >>
+        subgoal `I' (4,SUC t) = I' (3,t)` >-
+         (fs [is_sch_def,is_sch_memory_def,Abbr `s`] >>
+          `enable_stg 4 (agp32 fext fbits t)`
+            by fs [enable_stg_def,agp32_ID_ID_write_enable_MEM_state_flag] >>
+          Cases_on `isMemOp_hw_op (agp32 fext fbits t)` >>
+          fs [enable_stg_def] >>
+          METIS_TAC [MEM_stg_op_agp32_ID_EX_write_disable,
+                     agp32_ID_ID_write_enable_and_ID_EX_write_enable]) >> fs [] >>
+        subgoal `I' (3,SUC t) = I' (2,t)` >-
+         (fs [is_sch_def,is_sch_execute_def,Abbr `s`] >>
+          `enable_stg 3 (agp32 fext fbits t)`
+            by fs [enable_stg_def,agp32_ID_ID_write_enable_and_ID_EX_write_enable] >>
+          Cases_on `isJump_isa_op (I' (3,t)) a` >-
+           METIS_TAC [isJump_isa_op_not_none] >>
+          Cases_on `~reg_data_hazard (agp32 fext fbits t)` >>
+          METIS_TAC []) >> fs [] >>
+        `THE (I' (2,t)) = THE (I' (5,t)) + 1`
+          by METIS_TAC [EX_MEM_NONE_ID_instr_index_with_WB_instr_plus_1] >>
+        `THE (I' (5,t)) = THE (I' (2,t)) - 1` by fs [] >>
+        `THE (I' (1,t)) = THE (I' (2,t)) + 1`
+          by METIS_TAC [IF_instr_index_with_ID_instr_plus_1] >> fs [] >>
+        METIS_TAC [reg_adr_update_isa_not_change_data]) >>
+      `I' (2,SUC t) = I' (2,t)` by fs [is_sch_def,is_sch_disable_def] >>
+      subgoal `I' (5,SUC t) = I' (4,t)` >-
+       (fs [is_sch_def,is_sch_writeback_def,is_sch_disable_def,Abbr `s`] >>
+        Cases_on `enable_stg 5 (agp32 fext fbits t)` >>
+        METIS_TAC []) >> fs [] >>
+      Cases_on `enable_stg 3 (agp32 fext fbits t)` >-
+       (subgoal `I' (4,SUC t) = I' (3,t)` >-
+         (fs [is_sch_def,is_sch_memory_def,Abbr `s`] >>
+          `enable_stg 4 (agp32 fext fbits t)`
+            by fs [enable_stg_def,agp32_MEM_state_flag_eq_WB_state_flag] >>
+          Cases_on `isMemOp_hw_op (agp32 fext fbits t)` >>
+          fs [enable_stg_def] >>
+          METIS_TAC [MEM_stg_op_agp32_ID_EX_write_disable,enable_stg_def]) >> fs [] >>
+        `THE (I' (2,t)) = THE (I' (5,t)) + 1`
+          by METIS_TAC [EX_MEM_NONE_ID_instr_index_with_WB_instr_plus_1] >> fs []) >>
+      `I' (3,SUC t) = I' (3,t)` by METIS_TAC [is_sch_def,is_sch_disable_def] >> fs [] >>
+      `THE (I' (3,t)) = THE (I' (5,t)) + 1`
+        by METIS_TAC [EX_instr_index_with_WB_instr_plus_1_MEM_NONE] >>
+      `THE (I' (5,t)) = THE (I' (3,t)) - 1` by fs [] >>
+      `THE (I' (2,t)) = THE (I' (3,t)) + 1`
+        by METIS_TAC [ID_instr_index_with_EX_instr_plus_1] >> fs [] >>
+      METIS_TAC [reg_adr_update_isa_not_change_data]) >>
+    `~enable_stg 5 (agp32 fext fbits t)` by fs [enable_stg_def] >>
+    `I' (5,SUC t) = I' (5,t)` by METIS_TAC [is_sch_def,is_sch_disable_def] >> fs []) >-
    (** I (4,SUC t) and I (5,t) are not NONE **)
-   (`s.WB.WB_state_flag` by fs [Abbr `s`,enable_stg_def,agp32_ID_ID_write_enable_WB_state_flag] >>
-    `wb_data_vaild s` by fs [Abbr `s`,wb_data_vaild_def] >>
-    `(agp32 fext fbits (SUC t)).R = (FUNPOW Next (THE (I' (5,t))) a).R` by cheat >> fs [] >>
-    `(agp32 fext fbits (SUC t)).ID.ID_addrA = (22 >< 17) i`
-      by (fs [Abbr `i`,Abbr `s`,is_sch_def] >>
-          METIS_TAC [agp32_Rel_ag32_ID_addr_correct,addrA_def]) >> fs [] >>
-    subgoal `THE (I' (4,SUC t)) = THE (I' (5,t)) + 1` >-
-     (`I' (5,SUC t) = I' (4,t)`
+   (Cases_on`s.WB.WB_state_flag` >-
+     (`wb_data_vaild s` by fs [Abbr `s`,wb_data_vaild_def] >>
+      `(agp32 fext fbits (SUC t)).R = (FUNPOW Next (THE (I' (5,t))) a).R` by cheat >> fs [] >>
+      `(agp32 fext fbits (SUC t)).ID.ID_addrA = (22 >< 17) i`
+        by (fs [Abbr `i`,Abbr `s`,is_sch_def] >>
+            METIS_TAC [agp32_Rel_ag32_ID_addr_correct,addrA_def]) >> fs [] >>
+      Cases_on `enable_stg 2 (agp32 fext fbits t)` >-
+       (subgoal `THE (I' (4,SUC t)) = THE (I' (5,t)) + 1` >-
+         (`I' (5,SUC t) = I' (4,t)`
+            by (fs [is_sch_def,is_sch_writeback_def,is_sch_disable_def,Abbr `s`] >>
+                Cases_on `enable_stg 5 (agp32 fext fbits t)` >>
+                METIS_TAC []) >>
+          `I' (4,SUC t) = I' (3,t)`
+            by (fs [is_sch_def,is_sch_memory_def,Abbr `s`] >>
+                `enable_stg 4 (agp32 fext fbits t)`
+                  by fs [enable_stg_def,agp32_ID_ID_write_enable_MEM_state_flag] >>
+                Cases_on `isMemOp_hw_op (agp32 fext fbits t)` >>
+                fs [enable_stg_def] >>
+                METIS_TAC [MEM_stg_op_agp32_ID_EX_write_disable,
+                           agp32_ID_ID_write_enable_and_ID_EX_write_enable]) >> fs [] >>
+          METIS_TAC [EX_instr_index_with_WB_instr_plus_1_MEM_NONE]) >>
+        `THE (I' (5,t)) = THE (I' (4,SUC t)) - 1` by fs [] >> fs [] >>
+        `(FUNPOW Next (THE (I' (4,SUC t)) − 1) a).R ((22 >< 17) i) =
+        (FUNPOW Next (THE (I' (4,SUC t))) a).R ((22 >< 17) i)`
+          by METIS_TAC [reg_adr_update_isa_not_change_data] >> fs [] >>
+        `THE (I' (2,SUC t)) = THE (I' (4,SUC t)) + 1`
+          by METIS_TAC [EX_NONE_ID_instr_index_with_MEM_instr_plus_1] >> fs []) >>
+      `I' (2,SUC t) = I' (2,t)` by fs [is_sch_def,is_sch_disable_def] >>
+      subgoal `I' (4,SUC t) = I' (3,t)` >-
+       (fs [is_sch_def,is_sch_memory_def] >>
+        `enable_stg 4 (agp32 fext fbits t)`
+          by fs [enable_stg_def,agp32_MEM_state_flag_eq_WB_state_flag] >>
+        Cases_on `isMemOp_hw_op (agp32 fext fbits t)` >- METIS_TAC [] >> fs []) >>
+      `I' (5,SUC t) = I' (4,t)`
         by (fs [is_sch_def,is_sch_writeback_def,is_sch_disable_def,Abbr `s`] >>
             Cases_on `enable_stg 5 (agp32 fext fbits t)` >>
-            METIS_TAC []) >>
-      `I' (4,SUC t) = I' (3,t)`
-          by (fs [is_sch_def,is_sch_memory_def,Abbr `s`] >>
-              `enable_stg 4 (agp32 fext fbits t)`
-                by fs [enable_stg_def,agp32_ID_ID_write_enable_MEM_state_flag] >>
-              Cases_on `isMemOp_hw_op (agp32 fext fbits t)` >>
-              fs [enable_stg_def] >>
-              METIS_TAC [MEM_stg_op_agp32_ID_EX_write_disable,
-                         agp32_ID_ID_write_enable_and_ID_EX_write_enable]) >> fs [] >>
-      METIS_TAC [EX_instr_index_with_WB_instr_plus_1_MEM_NONE]) >>
-    `THE (I' (5,t)) = THE (I' (4,SUC t)) - 1` by fs [] >> fs [] >>
-    `(FUNPOW Next (THE (I' (4,SUC t)) − 1) a).R ((22 >< 17) i) =
-    (FUNPOW Next (THE (I' (4,SUC t))) a).R ((22 >< 17) i)`
-      by METIS_TAC [reg_adr_update_isa_not_change_data] >> fs [] >>
-    `THE (I' (2,SUC t)) = THE (I' (4,SUC t)) + 1`
-      by METIS_TAC [EX_NONE_ID_instr_index_with_MEM_instr_plus_1] >> fs []) >-
+            METIS_TAC []) >> fs [] >>
+      `THE (I' (3,t)) = THE (I' (5,t)) + 1`
+        by METIS_TAC [EX_instr_index_with_WB_instr_plus_1_MEM_NONE] >>
+      `THE (I' (5,t)) = THE (I' (3,t)) - 1` by fs [] >>
+      `THE (I' (2,t)) = THE (I' (3,t)) + 1`
+        by METIS_TAC [ID_instr_index_with_EX_instr_plus_1] >> fs [] >>
+      METIS_TAC [reg_adr_update_isa_not_change_data]) >>
+    `~enable_stg 5 (agp32 fext fbits t)` by fs [enable_stg_def] >>
+    `I' (5,SUC t) = I' (5,t)` by METIS_TAC [is_sch_def,is_sch_disable_def] >> fs []) >-     
    (** I (3,SUC t), I (4,SUC t) and I (5,t) are not NONE **)
-   (`s.WB.WB_state_flag` by fs [Abbr `s`,enable_stg_def,agp32_ID_ID_write_enable_WB_state_flag] >>
-    `wb_data_vaild s` by fs [Abbr `s`,wb_data_vaild_def] >>
+   (Cases_on `s.WB.WB_state_flag` >-
+     (`wb_data_vaild s` by fs [Abbr `s`,wb_data_vaild_def] >>
+      `(agp32 fext fbits (SUC t)).R = (FUNPOW Next (THE (I' (5,t))) a).R` by cheat >> fs [] >>
+      `(agp32 fext fbits (SUC t)).ID.ID_addrA = (22 >< 17) i`
+        by (fs [Abbr `i`,Abbr `s`,is_sch_def] >>
+            METIS_TAC [agp32_Rel_ag32_ID_addr_correct,addrA_def]) >> fs [] >>
+      Cases_on `enable_stg 2 (agp32 fext fbits t)` >-
+       (subgoal `THE (I' (4,SUC t)) = THE (I' (5,t)) + 1` >-
+         (`I' (5,SUC t) = I' (4,t)`
+            by (fs [is_sch_def,is_sch_writeback_def,is_sch_disable_def,Abbr `s`] >>
+                Cases_on `enable_stg 5 (agp32 fext fbits t)` >>
+                METIS_TAC []) >>
+          `I' (4,SUC t) = I' (3,t)`
+            by (fs [is_sch_def,is_sch_memory_def,Abbr `s`] >>
+                `enable_stg 4 (agp32 fext fbits t)`
+                  by fs [enable_stg_def,agp32_ID_ID_write_enable_MEM_state_flag] >>
+                Cases_on `isMemOp_hw_op (agp32 fext fbits t)` >>
+                fs [enable_stg_def] >>
+                METIS_TAC [MEM_stg_op_agp32_ID_EX_write_disable,
+                           agp32_ID_ID_write_enable_and_ID_EX_write_enable]) >> fs [] >>
+          METIS_TAC [EX_instr_index_with_WB_instr_plus_1_MEM_NONE]) >>
+        `THE (I' (5,t)) = THE (I' (4,SUC t)) - 1` by fs [] >> fs [] >>
+        `(FUNPOW Next (THE (I' (4,SUC t)) − 1) a).R ((22 >< 17) i) =
+        (FUNPOW Next (THE (I' (4,SUC t))) a).R ((22 >< 17) i)`
+          by METIS_TAC [reg_adr_update_isa_not_change_data] >> fs [] >>
+        `THE (I' (3,SUC t)) = THE (I' (4,SUC t)) + 1`
+          by METIS_TAC [EX_instr_index_with_MEM_instr_plus_1] >>
+        `THE (I' (2,SUC t)) = THE (I' (3,SUC t)) + 1`
+          by METIS_TAC [ID_instr_index_with_EX_instr_plus_1] >> fs [] >>
+        `THE (I' (4,SUC t)) = THE (I' (3,SUC t)) - 1` by FULL_SIMP_TAC std_ss [] >>
+        METIS_TAC [reg_adr_update_isa_not_change_data]) >>
+      `I' (2,SUC t) = I' (2,t)` by fs [is_sch_def,is_sch_disable_def] >>
+      subgoal `I' (4,SUC t) = I' (3,t)` >-
+       (fs [is_sch_def,is_sch_memory_def] >>
+        `enable_stg 4 (agp32 fext fbits t)`
+          by fs [enable_stg_def,agp32_MEM_state_flag_eq_WB_state_flag] >>
+        Cases_on `isMemOp_hw_op (agp32 fext fbits t)` >- METIS_TAC [] >> fs []) >>
+      `I' (5,SUC t) = I' (4,t)`
+        by (fs [is_sch_def,is_sch_writeback_def,is_sch_disable_def,Abbr `s`] >>
+            Cases_on `enable_stg 5 (agp32 fext fbits t)` >>
+            METIS_TAC []) >> fs [] >>
+      `THE (I' (3,t)) = THE (I' (5,t)) + 1`
+        by METIS_TAC [EX_instr_index_with_WB_instr_plus_1_MEM_NONE] >>
+      `THE (I' (5,t)) = THE (I' (3,t)) - 1` by fs [] >>
+      `THE (I' (2,t)) = THE (I' (3,t)) + 1`
+        by METIS_TAC [ID_instr_index_with_EX_instr_plus_1] >> fs [] >>
+      METIS_TAC [reg_adr_update_isa_not_change_data]) >>
+    `~enable_stg 5 (agp32 fext fbits t)` by fs [enable_stg_def] >>
+    `I' (5,SUC t) = I' (5,t)` by METIS_TAC [is_sch_def,is_sch_disable_def] >> fs []) >-
+   (** I (5,SUC t) and I (5,t) are not NONE **)
+   (Cases_on `s.WB.WB_state_flag` >-
+    (`wb_data_vaild s` by fs [Abbr `s`,wb_data_vaild_def] >>
+     `(agp32 fext fbits (SUC t)).R = (FUNPOW Next (THE (I' (5,t))) a).R` by cheat >> fs [] >>
+     `(agp32 fext fbits (SUC t)).ID.ID_addrA = (22 >< 17) i`
+       by (fs [Abbr `i`,Abbr `s`,is_sch_def] >>
+           METIS_TAC [agp32_Rel_ag32_ID_addr_correct,addrA_def]) >> fs [] >>
+     `enable_stg 5 (agp32 fext fbits t)`
+       by fs [enable_stg_def,agp32_ID_ID_write_enable_WB_state_flag] >>
+     `THE (I' (5,SUC t)) = THE (I' (5,t)) + 1` by METIS_TAC [WB_instr_index_t_SUC_t_enable] >>
+     `THE (I' (5,t)) = THE (I' (5,SUC t)) - 1` by fs [] >> fs [] >>
+     `(FUNPOW Next (THE (I' (5,SUC t)) − 1) a).R ((22 >< 17) i) =
+     (FUNPOW Next (THE (I' (5,SUC t))) a).R ((22 >< 17) i)`
+       by METIS_TAC [reg_adr_update_isa_not_change_data] >> fs [] >>
+     `THE (I' (2,SUC t)) = THE (I' (5,SUC t)) + 1`
+       by METIS_TAC [EX_MEM_NONE_ID_instr_index_with_WB_instr_plus_1] >> fs []) >>
+    `~enable_stg 5 (agp32 fext fbits t)` by fs [enable_stg_def] >>
+    `~enable_stg 4 (agp32 fext fbits t)`
+      by fs [enable_stg_def,agp32_MEM_state_flag_eq_WB_state_flag] >>
+    `~(agp32 fext fbits t).ID.ID_ID_write_enable /\ ~(agp32 fext fbits t).ID.ID_EX_write_enable`
+      by METIS_TAC [agp32_ID_EX_write_enable_WB_state_flag,agp32_ID_ID_write_enable_WB_state_flag] >>
+    `~enable_stg 2 (agp32 fext fbits t) /\
+    ~enable_stg 3 (agp32 fext fbits t)` by fs [enable_stg_def] >>
+    `(agp32 fext fbits (SUC t)).ID.ID_addrA = s.ID.ID_addrA`
+      by METIS_TAC [Abbr `s`,is_sch_def,agp32_ID_disabled_ID_addr_unchanged] >>
+    `(agp32 fext fbits (SUC t)).ID.ID_addrA_disable = (agp32 fext fbits t).ID.ID_addrA_disable`
+      by METIS_TAC [Abbr `s`,is_sch_def,agp32_ID_disabled_ID_flag_unchanged] >>
+    `(agp32 fext fbits (SUC t)).ID.ID_read_dataA = (agp32 fext fbits t).ID.ID_read_dataA`
+      by METIS_TAC [Abbr `s`,is_sch_def,agp32_ID_disabled_ID_read_data_unchanged] >>
+    `(I' (2,SUC t) = I' (2,t)) /\ (I' (3,SUC t) = I' (3,t)) /\
+    (I' (4,SUC t) = I' (4,t)) /\ (I' (5,SUC t) = I' (5,t))` by METIS_TAC [is_sch_def,is_sch_disable_def] >>
+    fs [Rel_def,ID_reg_data_Rel_def,reg_dataA_def,addrA_def] >> METIS_TAC []) >-
+   (** I (3,SUC t), I (5,SUC t) and I (5,t) are not NONE **)
+   (Cases_on `s.WB.WB_state_flag` >-
+     (`wb_data_vaild s` by fs [Abbr `s`,wb_data_vaild_def] >>
+      `(agp32 fext fbits (SUC t)).R = (FUNPOW Next (THE (I' (5,t))) a).R` by cheat >> fs [] >>
+      `(agp32 fext fbits (SUC t)).ID.ID_addrA = (22 >< 17) i`
+        by (fs [Abbr `i`,Abbr `s`,is_sch_def] >>
+            METIS_TAC [agp32_Rel_ag32_ID_addr_correct,addrA_def]) >> fs [] >>
+      `enable_stg 5 (agp32 fext fbits t)`
+        by fs [enable_stg_def,agp32_ID_ID_write_enable_WB_state_flag] >>
+      `THE (I' (5,SUC t)) = THE (I' (5,t)) + 1` by METIS_TAC [WB_instr_index_t_SUC_t_enable] >>
+      `THE (I' (5,t)) = THE (I' (5,SUC t)) - 1` by fs [] >> fs [] >>
+      `(FUNPOW Next (THE (I' (5,SUC t)) − 1) a).R ((22 >< 17) i) =
+      (FUNPOW Next (THE (I' (5,SUC t))) a).R ((22 >< 17) i)`
+        by METIS_TAC [reg_adr_update_isa_not_change_data] >> fs [] >>
+      `THE (I' (3,SUC t)) = THE (I' (5,SUC t)) + 1`
+        by METIS_TAC [EX_instr_index_with_WB_instr_plus_1_MEM_NONE] >>
+      `THE (I' (2,SUC t)) = THE (I' (3,SUC t)) + 1`
+        by METIS_TAC [ID_instr_index_with_EX_instr_plus_1] >> fs [] >>
+      `THE (I' (5,SUC t)) = THE (I' (3,SUC t)) - 1` by fs [] >>
+      METIS_TAC [reg_adr_update_isa_not_change_data]) >>
+    `~enable_stg 5 (agp32 fext fbits t)` by fs [enable_stg_def] >>
+    `~enable_stg 4 (agp32 fext fbits t)`
+      by fs [enable_stg_def,agp32_MEM_state_flag_eq_WB_state_flag] >>
+    `~(agp32 fext fbits t).ID.ID_ID_write_enable /\ ~(agp32 fext fbits t).ID.ID_EX_write_enable`
+      by METIS_TAC [agp32_ID_EX_write_enable_WB_state_flag,agp32_ID_ID_write_enable_WB_state_flag] >>
+    `~enable_stg 2 (agp32 fext fbits t) /\
+    ~enable_stg 3 (agp32 fext fbits t)` by fs [enable_stg_def] >>
+    `(agp32 fext fbits (SUC t)).ID.ID_addrA = s.ID.ID_addrA`
+      by METIS_TAC [Abbr `s`,is_sch_def,agp32_ID_disabled_ID_addr_unchanged] >>
+    `(agp32 fext fbits (SUC t)).ID.ID_addrA_disable = (agp32 fext fbits t).ID.ID_addrA_disable`
+      by METIS_TAC [Abbr `s`,is_sch_def,agp32_ID_disabled_ID_flag_unchanged] >>
+    `(agp32 fext fbits (SUC t)).ID.ID_read_dataA = (agp32 fext fbits t).ID.ID_read_dataA`
+      by METIS_TAC [Abbr `s`,is_sch_def,agp32_ID_disabled_ID_read_data_unchanged] >>
+    `(I' (2,SUC t) = I' (2,t)) /\ (I' (3,SUC t) = I' (3,t)) /\
+    (I' (4,SUC t) = I' (4,t)) /\ (I' (5,SUC t) = I' (5,t))` by METIS_TAC [is_sch_def,is_sch_disable_def] >>
+    fs [Rel_def,ID_reg_data_Rel_def,reg_dataA_def,addrA_def] >> METIS_TAC []) >-
+   (** I (4,SUC t), I (5,SUC t) and I (5,t) are not NONE **)
+   (Cases_on `s.WB.WB_state_flag` >-
+     (`wb_data_vaild s` by fs [Abbr `s`,wb_data_vaild_def] >>
+      `(agp32 fext fbits (SUC t)).R = (FUNPOW Next (THE (I' (5,t))) a).R` by cheat >> fs [] >>
+      `(agp32 fext fbits (SUC t)).ID.ID_addrA = (22 >< 17) i`
+        by (fs [Abbr `i`,Abbr `s`,is_sch_def] >>
+            METIS_TAC [agp32_Rel_ag32_ID_addr_correct,addrA_def]) >> fs [] >>
+      `enable_stg 5 (agp32 fext fbits t)`
+        by fs [enable_stg_def,agp32_ID_ID_write_enable_WB_state_flag] >>
+      `THE (I' (5,SUC t)) = THE (I' (5,t)) + 1` by METIS_TAC [WB_instr_index_t_SUC_t_enable] >>
+      `THE (I' (5,t)) = THE (I' (5,SUC t)) - 1` by fs [] >> fs [] >>
+      `(FUNPOW Next (THE (I' (5,SUC t)) − 1) a).R ((22 >< 17) i) =
+      (FUNPOW Next (THE (I' (5,SUC t))) a).R ((22 >< 17) i)`
+        by METIS_TAC [reg_adr_update_isa_not_change_data] >> fs [] >>
+      `THE (I' (4,SUC t)) = THE (I' (5,SUC t)) + 1`
+        by METIS_TAC [MEM_instr_index_with_WB_instr_plus_1] >>
+      `THE (I' (2,SUC t)) = THE (I' (4,SUC t)) + 1`
+        by METIS_TAC [EX_NONE_ID_instr_index_with_MEM_instr_plus_1] >> fs [] >>
+      `THE (I' (5,SUC t)) = THE (I' (4,SUC t)) - 1` by fs [] >>
+      METIS_TAC [reg_adr_update_isa_not_change_data]) >>
+    `~enable_stg 5 (agp32 fext fbits t)` by fs [enable_stg_def] >>
+    `~enable_stg 4 (agp32 fext fbits t)`
+      by fs [enable_stg_def,agp32_MEM_state_flag_eq_WB_state_flag] >>
+    `~(agp32 fext fbits t).ID.ID_ID_write_enable /\ ~(agp32 fext fbits t).ID.ID_EX_write_enable`
+      by METIS_TAC [agp32_ID_EX_write_enable_WB_state_flag,agp32_ID_ID_write_enable_WB_state_flag] >>
+    `~enable_stg 2 (agp32 fext fbits t) /\
+    ~enable_stg 3 (agp32 fext fbits t)` by fs [enable_stg_def] >>
+    `(agp32 fext fbits (SUC t)).ID.ID_addrA = s.ID.ID_addrA`
+      by METIS_TAC [Abbr `s`,is_sch_def,agp32_ID_disabled_ID_addr_unchanged] >>
+    `(agp32 fext fbits (SUC t)).ID.ID_addrA_disable = (agp32 fext fbits t).ID.ID_addrA_disable`
+      by METIS_TAC [Abbr `s`,is_sch_def,agp32_ID_disabled_ID_flag_unchanged] >>
+    `(agp32 fext fbits (SUC t)).ID.ID_read_dataA = (agp32 fext fbits t).ID.ID_read_dataA`
+      by METIS_TAC [Abbr `s`,is_sch_def,agp32_ID_disabled_ID_read_data_unchanged] >>
+    `(I' (2,SUC t) = I' (2,t)) /\ (I' (3,SUC t) = I' (3,t)) /\
+    (I' (4,SUC t) = I' (4,t)) /\ (I' (5,SUC t) = I' (5,t))` by METIS_TAC [is_sch_def,is_sch_disable_def] >>
+    fs [Rel_def,ID_reg_data_Rel_def,reg_dataA_def,addrA_def] >> METIS_TAC []) >>
+  (** all are not NONE **)
+  Cases_on `s.WB.WB_state_flag` >-
+   (`wb_data_vaild s` by fs [Abbr `s`,wb_data_vaild_def] >>
     `(agp32 fext fbits (SUC t)).R = (FUNPOW Next (THE (I' (5,t))) a).R` by cheat >> fs [] >>
     `(agp32 fext fbits (SUC t)).ID.ID_addrA = (22 >< 17) i`
       by (fs [Abbr `i`,Abbr `s`,is_sch_def] >>
           METIS_TAC [agp32_Rel_ag32_ID_addr_correct,addrA_def]) >> fs [] >>
-    subgoal `THE (I' (4,SUC t)) = THE (I' (5,t)) + 1` >-
-     (`I' (5,SUC t) = I' (4,t)`
-        by (fs [is_sch_def,is_sch_writeback_def,is_sch_disable_def,Abbr `s`] >>
-            Cases_on `enable_stg 5 (agp32 fext fbits t)` >>
-            METIS_TAC []) >>
-      `I' (4,SUC t) = I' (3,t)`
-          by (fs [is_sch_def,is_sch_memory_def,Abbr `s`] >>
-              `enable_stg 4 (agp32 fext fbits t)`
-                by fs [enable_stg_def,agp32_ID_ID_write_enable_MEM_state_flag] >>
-              Cases_on `isMemOp_hw_op (agp32 fext fbits t)` >>
-              fs [enable_stg_def] >>
-              METIS_TAC [MEM_stg_op_agp32_ID_EX_write_disable,
-                         agp32_ID_ID_write_enable_and_ID_EX_write_enable]) >> fs [] >>
-      METIS_TAC [EX_instr_index_with_WB_instr_plus_1_MEM_NONE]) >>
-    `THE (I' (5,t)) = THE (I' (4,SUC t)) - 1` by fs [] >> fs [] >>
+    `enable_stg 5 (agp32 fext fbits t)`
+      by fs [enable_stg_def,agp32_ID_ID_write_enable_WB_state_flag] >>
+    `THE (I' (5,SUC t)) = THE (I' (5,t)) + 1` by METIS_TAC [WB_instr_index_t_SUC_t_enable] >>
+    `THE (I' (5,t)) = THE (I' (5,SUC t)) - 1` by fs [] >> fs [] >>
+    `(FUNPOW Next (THE (I' (5,SUC t)) − 1) a).R ((22 >< 17) i) =
+    (FUNPOW Next (THE (I' (5,SUC t))) a).R ((22 >< 17) i)`
+      by METIS_TAC [reg_adr_update_isa_not_change_data] >> fs [] >>
+    qpat_x_assum `THE (I' (5,SUC t)) = _` (fn thm => all_tac)  >>
+    `THE (I' (4,SUC t)) = THE (I' (5,SUC t)) + 1`
+      by METIS_TAC [MEM_instr_index_with_WB_instr_plus_1] >>
+    `THE (I' (5,SUC t)) = THE (I' (4,SUC t)) - 1` by fs [] >> fs [] >>
     `(FUNPOW Next (THE (I' (4,SUC t)) − 1) a).R ((22 >< 17) i) =
     (FUNPOW Next (THE (I' (4,SUC t))) a).R ((22 >< 17) i)`
       by METIS_TAC [reg_adr_update_isa_not_change_data] >> fs [] >>
@@ -937,90 +1215,23 @@ Proof
     `THE (I' (2,SUC t)) = THE (I' (3,SUC t)) + 1`
       by METIS_TAC [ID_instr_index_with_EX_instr_plus_1] >> fs [] >>
     `THE (I' (4,SUC t)) = THE (I' (3,SUC t)) - 1` by FULL_SIMP_TAC std_ss [] >>
-    METIS_TAC [reg_adr_update_isa_not_change_data]) >-
-   (** I (5,SUC t) and I (5,t) are not NONE **)
-   (`s.WB.WB_state_flag` by fs [Abbr `s`,enable_stg_def,agp32_ID_ID_write_enable_WB_state_flag] >>
-    `wb_data_vaild s` by fs [Abbr `s`,wb_data_vaild_def] >>
-    `(agp32 fext fbits (SUC t)).R = (FUNPOW Next (THE (I' (5,t))) a).R` by cheat >> fs [] >>
-    `(agp32 fext fbits (SUC t)).ID.ID_addrA = (22 >< 17) i`
-      by (fs [Abbr `i`,Abbr `s`,is_sch_def] >>
-          METIS_TAC [agp32_Rel_ag32_ID_addr_correct,addrA_def]) >> fs [] >>
-    `enable_stg 5 (agp32 fext fbits t)`
-      by fs [enable_stg_def,agp32_ID_ID_write_enable_WB_state_flag] >>
-    `THE (I' (5,SUC t)) = THE (I' (5,t)) + 1` by METIS_TAC [WB_instr_index_t_SUC_t_enable] >>
-    `THE (I' (5,t)) = THE (I' (5,SUC t)) - 1` by fs [] >> fs [] >>
-    `(FUNPOW Next (THE (I' (5,SUC t)) − 1) a).R ((22 >< 17) i) =
-    (FUNPOW Next (THE (I' (5,SUC t))) a).R ((22 >< 17) i)`
-      by METIS_TAC [reg_adr_update_isa_not_change_data] >> fs [] >>
-    `THE (I' (2,SUC t)) = THE (I' (5,SUC t)) + 1`
-      by METIS_TAC [EX_MEM_NONE_ID_instr_index_with_WB_instr_plus_1] >> fs []) >-
-   (** I (3,SUC t), I (5,SUC t) and I (5,t) are not NONE **)
-   (`s.WB.WB_state_flag` by fs [Abbr `s`,enable_stg_def,agp32_ID_ID_write_enable_WB_state_flag] >>
-    `wb_data_vaild s` by fs [Abbr `s`,wb_data_vaild_def] >>
-    `(agp32 fext fbits (SUC t)).R = (FUNPOW Next (THE (I' (5,t))) a).R` by cheat >> fs [] >>
-    `(agp32 fext fbits (SUC t)).ID.ID_addrA = (22 >< 17) i`
-      by (fs [Abbr `i`,Abbr `s`,is_sch_def] >>
-          METIS_TAC [agp32_Rel_ag32_ID_addr_correct,addrA_def]) >> fs [] >>
-    `enable_stg 5 (agp32 fext fbits t)`
-      by fs [enable_stg_def,agp32_ID_ID_write_enable_WB_state_flag] >>
-    `THE (I' (5,SUC t)) = THE (I' (5,t)) + 1` by METIS_TAC [WB_instr_index_t_SUC_t_enable] >>
-    `THE (I' (5,t)) = THE (I' (5,SUC t)) - 1` by fs [] >> fs [] >>
-    `(FUNPOW Next (THE (I' (5,SUC t)) − 1) a).R ((22 >< 17) i) =
-    (FUNPOW Next (THE (I' (5,SUC t))) a).R ((22 >< 17) i)`
-      by METIS_TAC [reg_adr_update_isa_not_change_data] >> fs [] >>
-    `THE (I' (3,SUC t)) = THE (I' (5,SUC t)) + 1`
-      by METIS_TAC [EX_instr_index_with_WB_instr_plus_1_MEM_NONE] >>
-    `THE (I' (2,SUC t)) = THE (I' (3,SUC t)) + 1`
-      by METIS_TAC [ID_instr_index_with_EX_instr_plus_1] >> fs [] >>
-    `THE (I' (5,SUC t)) = THE (I' (3,SUC t)) - 1` by fs [] >>
-    METIS_TAC [reg_adr_update_isa_not_change_data]) >-
-   (** I (4,SUC t), I (5,SUC t) and I (5,t) are not NONE **)
-   (`s.WB.WB_state_flag` by fs [Abbr `s`,enable_stg_def,agp32_ID_ID_write_enable_WB_state_flag] >>
-    `wb_data_vaild s` by fs [Abbr `s`,wb_data_vaild_def] >>
-    `(agp32 fext fbits (SUC t)).R = (FUNPOW Next (THE (I' (5,t))) a).R` by cheat >> fs [] >>
-    `(agp32 fext fbits (SUC t)).ID.ID_addrA = (22 >< 17) i`
-      by (fs [Abbr `i`,Abbr `s`,is_sch_def] >>
-          METIS_TAC [agp32_Rel_ag32_ID_addr_correct,addrA_def]) >> fs [] >>
-    `enable_stg 5 (agp32 fext fbits t)`
-      by fs [enable_stg_def,agp32_ID_ID_write_enable_WB_state_flag] >>
-    `THE (I' (5,SUC t)) = THE (I' (5,t)) + 1` by METIS_TAC [WB_instr_index_t_SUC_t_enable] >>
-    `THE (I' (5,t)) = THE (I' (5,SUC t)) - 1` by fs [] >> fs [] >>
-    `(FUNPOW Next (THE (I' (5,SUC t)) − 1) a).R ((22 >< 17) i) =
-    (FUNPOW Next (THE (I' (5,SUC t))) a).R ((22 >< 17) i)`
-      by METIS_TAC [reg_adr_update_isa_not_change_data] >> fs [] >>
-    `THE (I' (4,SUC t)) = THE (I' (5,SUC t)) + 1`
-      by METIS_TAC [MEM_instr_index_with_WB_instr_plus_1] >>
-    `THE (I' (2,SUC t)) = THE (I' (4,SUC t)) + 1`
-      by METIS_TAC [EX_NONE_ID_instr_index_with_MEM_instr_plus_1] >> fs [] >>
-    `THE (I' (5,SUC t)) = THE (I' (4,SUC t)) - 1` by fs [] >>
     METIS_TAC [reg_adr_update_isa_not_change_data]) >>
-  (** all are not NONE **)
-  `s.WB.WB_state_flag` by fs [Abbr `s`,enable_stg_def,agp32_ID_ID_write_enable_WB_state_flag] >>
-  `wb_data_vaild s` by fs [Abbr `s`,wb_data_vaild_def] >>
-  `(agp32 fext fbits (SUC t)).R = (FUNPOW Next (THE (I' (5,t))) a).R` by cheat >> fs [] >>
-  `(agp32 fext fbits (SUC t)).ID.ID_addrA = (22 >< 17) i`
-    by (fs [Abbr `i`,Abbr `s`,is_sch_def] >>
-        METIS_TAC [agp32_Rel_ag32_ID_addr_correct,addrA_def]) >> fs [] >>
-  `enable_stg 5 (agp32 fext fbits t)`
-    by fs [enable_stg_def,agp32_ID_ID_write_enable_WB_state_flag] >>
-  `THE (I' (5,SUC t)) = THE (I' (5,t)) + 1` by METIS_TAC [WB_instr_index_t_SUC_t_enable] >>
-  `THE (I' (5,t)) = THE (I' (5,SUC t)) - 1` by fs [] >> fs [] >>
-  `(FUNPOW Next (THE (I' (5,SUC t)) − 1) a).R ((22 >< 17) i) =
-  (FUNPOW Next (THE (I' (5,SUC t))) a).R ((22 >< 17) i)`
-    by METIS_TAC [reg_adr_update_isa_not_change_data] >> fs [] >>
-  qpat_x_assum `THE (I' (5,SUC t)) = _` (fn thm => all_tac)  >>
-  `THE (I' (4,SUC t)) = THE (I' (5,SUC t)) + 1`
-    by METIS_TAC [MEM_instr_index_with_WB_instr_plus_1] >>
-  `THE (I' (5,SUC t)) = THE (I' (4,SUC t)) - 1` by fs [] >> fs [] >>
-  `(FUNPOW Next (THE (I' (4,SUC t)) − 1) a).R ((22 >< 17) i) =
-  (FUNPOW Next (THE (I' (4,SUC t))) a).R ((22 >< 17) i)`
-    by METIS_TAC [reg_adr_update_isa_not_change_data] >> fs [] >>
-  `THE (I' (3,SUC t)) = THE (I' (4,SUC t)) + 1`
-    by METIS_TAC [EX_instr_index_with_MEM_instr_plus_1] >>
-  `THE (I' (2,SUC t)) = THE (I' (3,SUC t)) + 1`
-    by METIS_TAC [ID_instr_index_with_EX_instr_plus_1] >> fs [] >>
-  `THE (I' (4,SUC t)) = THE (I' (3,SUC t)) - 1` by FULL_SIMP_TAC std_ss [] >>
-  METIS_TAC [reg_adr_update_isa_not_change_data]
+  `~enable_stg 5 (agp32 fext fbits t)` by fs [enable_stg_def] >>
+  `~enable_stg 4 (agp32 fext fbits t)`
+    by fs [enable_stg_def,agp32_MEM_state_flag_eq_WB_state_flag] >>
+  `~(agp32 fext fbits t).ID.ID_ID_write_enable /\ ~(agp32 fext fbits t).ID.ID_EX_write_enable`
+    by METIS_TAC [agp32_ID_EX_write_enable_WB_state_flag,agp32_ID_ID_write_enable_WB_state_flag] >>
+  `~enable_stg 2 (agp32 fext fbits t) /\
+  ~enable_stg 3 (agp32 fext fbits t)` by fs [enable_stg_def] >>
+  `(agp32 fext fbits (SUC t)).ID.ID_addrA = s.ID.ID_addrA`
+    by METIS_TAC [Abbr `s`,is_sch_def,agp32_ID_disabled_ID_addr_unchanged] >>
+  `(agp32 fext fbits (SUC t)).ID.ID_addrA_disable = (agp32 fext fbits t).ID.ID_addrA_disable`
+    by METIS_TAC [Abbr `s`,is_sch_def,agp32_ID_disabled_ID_flag_unchanged] >>
+  `(agp32 fext fbits (SUC t)).ID.ID_read_dataA = (agp32 fext fbits t).ID.ID_read_dataA`
+    by METIS_TAC [Abbr `s`,is_sch_def,agp32_ID_disabled_ID_read_data_unchanged] >>
+  `(I' (2,SUC t) = I' (2,t)) /\ (I' (3,SUC t) = I' (3,t)) /\
+  (I' (4,SUC t) = I' (4,t)) /\ (I' (5,SUC t) = I' (5,t))` by METIS_TAC [is_sch_def,is_sch_disable_def] >>
+  fs [Rel_def,ID_reg_data_Rel_def,reg_dataA_def,addrA_def] >> METIS_TAC []
 QED
 
 
@@ -1029,8 +1240,8 @@ Theorem agp32_Rel_ag32_ID_read_dataB_no_write_before:
   !fext fbits a t I.
     is_sch I (agp32 fext fbits) a ==>
     Rel I (fext t) (agp32 fext fbits (t-1)) (agp32 fext fbits t) a t ==>
-    enable_stg 2 (agp32 fext fbits t) ==>
     I (2,SUC t) <> NONE ==>
+    ~(agp32 fext fbits (SUC t)).ID.ID_addrB_disable ==>
     ~reg_adr_update_isa (I (3,SUC t)) a (agp32 fext fbits (SUC t)).ID.ID_addrB ==>
     ~reg_adr_update_isa (I (4,SUC t)) a (agp32 fext fbits (SUC t)).ID.ID_addrB ==>
     ~reg_adr_update_isa (I (5,SUC t)) a (agp32 fext fbits (SUC t)).ID.ID_addrB ==>
@@ -1156,123 +1367,336 @@ Proof
     `THE (I' (4,SUC t)) = THE (I' (3,SUC t)) - 1` by FULL_SIMP_TAC std_ss [] >>
     METIS_TAC [reg_adr_update_isa_not_change_data]) >-
    (** I (5,t) is not NONE **)
-   (`s.WB.WB_state_flag` by fs [Abbr `s`,enable_stg_def,agp32_ID_ID_write_enable_WB_state_flag] >>
-    `wb_data_vaild s` by fs [Abbr `s`,wb_data_vaild_def] >>
-    `(agp32 fext fbits (SUC t)).R = (FUNPOW Next (THE (I' (5,t))) a).R` by cheat >> fs [] >>
-    subgoal `I' (2,SUC t) = I' (1,t)` >-
-     (fs [is_sch_def,is_sch_decode_def,Abbr `s`] >>
-      Cases_on `isJump_isa_op (I' (2,t)) a \/ isJump_isa_op (I' (3,t)) a` >>
-      METIS_TAC []) >> fs [] >>
-    subgoal `I' (5,SUC t) = I' (4,t)` >-
-     (fs [is_sch_def,is_sch_writeback_def,is_sch_disable_def,Abbr `s`] >>
-      Cases_on `enable_stg 5 (agp32 fext fbits t)` >>
-      METIS_TAC []) >> fs [] >>
-    subgoal `I' (4,SUC t) = I' (3,t)` >-
-     (fs [is_sch_def,is_sch_memory_def,Abbr `s`] >>
-      `enable_stg 4 (agp32 fext fbits t)`
-        by fs [enable_stg_def,agp32_ID_ID_write_enable_MEM_state_flag] >>
-      Cases_on `isMemOp_hw_op (agp32 fext fbits t)` >>
-      fs [enable_stg_def] >>
-      METIS_TAC [MEM_stg_op_agp32_ID_EX_write_disable,
-                 agp32_ID_ID_write_enable_and_ID_EX_write_enable]) >> fs [] >>
-    subgoal `I' (3,SUC t) = I' (2,t)` >-
-     (fs [is_sch_def,is_sch_execute_def,Abbr `s`] >>
-      `enable_stg 3 (agp32 fext fbits t)`
-        by fs [enable_stg_def,agp32_ID_ID_write_enable_and_ID_EX_write_enable] >>
-      Cases_on `isJump_hw_op (agp32 fext fbits t)` >-
-       (`isJump_isa_op (I' (3,t)) a` by fs [isJump_hw_op_def,Rel_def,EX_Rel_spec_def] >>
-         METIS_TAC [isJump_isa_op_not_none]) >>
-      Cases_on `~reg_data_hazard (agp32 fext fbits t)` >- METIS_TAC [] >>
-      fs [isJump_hw_op_def,enable_stg_def] >>
-      METIS_TAC [agp32_ID_ID_write_enable_EX_jump_sel_then_no_reg_data_hazard]) >> fs [] >>
-    `THE (I' (1,t)) = THE (I' (5,t)) + 1`
-      by METIS_TAC [ID_EX_MEM_NONE_IF_instr_index_with_WB_instr_plus_1] >> fs []) >-
+   (Cases_on `s.WB.WB_state_flag` >-
+     (`wb_data_vaild s` by fs [Abbr `s`,wb_data_vaild_def] >>
+      `(agp32 fext fbits (SUC t)).R = (FUNPOW Next (THE (I' (5,t))) a).R` by cheat >> fs [] >>
+      Cases_on `enable_stg 2 (agp32 fext fbits t)` >-
+       (subgoal `I' (2,SUC t) = I' (1,t)` >-
+         (fs [is_sch_def,is_sch_decode_def,Abbr `s`] >>
+          METIS_TAC []) >> fs [] >>
+        subgoal `I' (5,SUC t) = I' (4,t)` >-
+         (fs [is_sch_def,is_sch_writeback_def,is_sch_disable_def,Abbr `s`] >>
+          Cases_on `enable_stg 5 (agp32 fext fbits t)` >>
+          METIS_TAC []) >> fs [] >>
+        subgoal `I' (4,SUC t) = I' (3,t)` >-
+         (fs [is_sch_def,is_sch_memory_def,Abbr `s`] >>
+          `enable_stg 4 (agp32 fext fbits t)`
+            by fs [enable_stg_def,agp32_ID_ID_write_enable_MEM_state_flag] >>
+          Cases_on `isMemOp_hw_op (agp32 fext fbits t)` >>
+          fs [enable_stg_def] >>
+          METIS_TAC [MEM_stg_op_agp32_ID_EX_write_disable,
+                     agp32_ID_ID_write_enable_and_ID_EX_write_enable]) >> fs [] >>
+        subgoal `I' (3,SUC t) = I' (2,t)` >-
+         (fs [is_sch_def,is_sch_execute_def,Abbr `s`] >>
+          `enable_stg 3 (agp32 fext fbits t)`
+            by fs [enable_stg_def,agp32_ID_ID_write_enable_and_ID_EX_write_enable] >>
+          Cases_on `isJump_hw_op (agp32 fext fbits t)` >-
+           (`isJump_isa_op (I' (3,t)) a` by fs [isJump_hw_op_def,Rel_def,EX_Rel_spec_def] >>
+            METIS_TAC [isJump_isa_op_not_none]) >>
+          Cases_on `~reg_data_hazard (agp32 fext fbits t)` >- METIS_TAC [] >>
+          fs [isJump_hw_op_def,enable_stg_def] >>
+          METIS_TAC [agp32_ID_ID_write_enable_EX_jump_sel_then_no_reg_data_hazard]) >> fs [] >>
+        `THE (I' (1,t)) = THE (I' (5,t)) + 1`
+          by METIS_TAC [ID_EX_MEM_NONE_IF_instr_index_with_WB_instr_plus_1] >> fs []) >>
+      `I' (2,SUC t) = I' (2,t)` by fs [is_sch_def,is_sch_disable_def] >>
+      subgoal `I' (5,SUC t) = I' (4,t)` >-
+       (fs [is_sch_def,is_sch_writeback_def,is_sch_disable_def,Abbr `s`] >>
+        Cases_on `enable_stg 5 (agp32 fext fbits t)` >>
+        METIS_TAC []) >> fs [] >>
+      Cases_on `enable_stg 3 (agp32 fext fbits t)` >-
+       (subgoal `I' (4,SUC t) = I' (3,t)` >-
+         (fs [is_sch_def,is_sch_memory_def,Abbr `s`] >>
+          `enable_stg 4 (agp32 fext fbits t)`
+            by fs [enable_stg_def,agp32_MEM_state_flag_eq_WB_state_flag] >>
+          Cases_on `isMemOp_hw_op (agp32 fext fbits t)` >>
+          fs [enable_stg_def] >>
+          METIS_TAC [MEM_stg_op_agp32_ID_EX_write_disable,enable_stg_def]) >> fs [] >>
+        `THE (I' (2,t)) = THE (I' (5,t)) + 1`
+          by METIS_TAC [EX_MEM_NONE_ID_instr_index_with_WB_instr_plus_1] >> fs []) >>
+      `I' (3,SUC t) = I' (3,t)` by METIS_TAC [is_sch_def,is_sch_disable_def] >>
+      `THE (I' (2,t)) = THE (I' (5,t)) + 1`
+        by METIS_TAC [EX_MEM_NONE_ID_instr_index_with_WB_instr_plus_1] >> fs []) >>
+    `~enable_stg 5 (agp32 fext fbits t)` by fs [enable_stg_def] >>
+    `I' (5,SUC t) = I' (5,t)` by METIS_TAC [is_sch_def,is_sch_disable_def] >> fs []) >-
    (** I (3,SUC t) and I (5,t) are not NONE **)
-   (`s.WB.WB_state_flag` by fs [Abbr `s`,enable_stg_def,agp32_ID_ID_write_enable_WB_state_flag] >>
-    `wb_data_vaild s` by fs [Abbr `s`,wb_data_vaild_def] >>
-    `(agp32 fext fbits (SUC t)).R = (FUNPOW Next (THE (I' (5,t))) a).R` by cheat >> fs [] >>
-    `(agp32 fext fbits (SUC t)).ID.ID_addrB = (15 >< 10) i`
-      by (fs [Abbr `i`,Abbr `s`,is_sch_def] >>
-          METIS_TAC [agp32_Rel_ag32_ID_addr_correct,addrB_def]) >> fs [] >>
-    subgoal `I' (2,SUC t) = I' (1,t)` >-
-     (fs [is_sch_def,is_sch_decode_def,Abbr `s`] >>
-      Cases_on `isJump_isa_op (I' (2,t)) a \/ isJump_isa_op (I' (3,t)) a` >>
-      METIS_TAC []) >> fs [] >>
-    subgoal `I' (5,SUC t) = I' (4,t)` >-
-     (fs [is_sch_def,is_sch_writeback_def,is_sch_disable_def,Abbr `s`] >>
-      Cases_on `enable_stg 5 (agp32 fext fbits t)` >>
-      METIS_TAC []) >> fs [] >>
-    subgoal `I' (4,SUC t) = I' (3,t)` >-
-     (fs [is_sch_def,is_sch_memory_def,Abbr `s`] >>
-      `enable_stg 4 (agp32 fext fbits t)`
-        by fs [enable_stg_def,agp32_ID_ID_write_enable_MEM_state_flag] >>
-      Cases_on `isMemOp_hw_op (agp32 fext fbits t)` >>
-      fs [enable_stg_def] >>
-      METIS_TAC [MEM_stg_op_agp32_ID_EX_write_disable,
-                 agp32_ID_ID_write_enable_and_ID_EX_write_enable]) >> fs [] >>
-     subgoal `I' (3,SUC t) = I' (2,t)` >-
-     (fs [is_sch_def,is_sch_execute_def,Abbr `s`] >>
-      `enable_stg 3 (agp32 fext fbits t)`
-        by fs [enable_stg_def,agp32_ID_ID_write_enable_and_ID_EX_write_enable] >>
-      Cases_on `isJump_isa_op (I' (3,t)) a` >-
-       METIS_TAC [isJump_isa_op_not_none] >>
-      Cases_on `~reg_data_hazard (agp32 fext fbits t)` >>
-      METIS_TAC []) >> fs [] >>
-    `THE (I' (2,t)) = THE (I' (5,t)) + 1`
-      by METIS_TAC [EX_MEM_NONE_ID_instr_index_with_WB_instr_plus_1] >>
-    `THE (I' (5,t)) = THE (I' (2,t)) - 1` by fs [] >>
-    `THE (I' (1,t)) = THE (I' (2,t)) + 1`
-      by METIS_TAC [IF_instr_index_with_ID_instr_plus_1] >> fs [] >>
-    METIS_TAC [reg_adr_update_isa_not_change_data]) >-
+   (Cases_on `s.WB.WB_state_flag` >-
+     (`wb_data_vaild s` by fs [Abbr `s`,wb_data_vaild_def] >>
+      `(agp32 fext fbits (SUC t)).R = (FUNPOW Next (THE (I' (5,t))) a).R` by cheat >> fs [] >>
+      `(agp32 fext fbits (SUC t)).ID.ID_addrB = (15 >< 10) i`
+        by (fs [Abbr `i`,Abbr `s`,is_sch_def] >>
+            METIS_TAC [agp32_Rel_ag32_ID_addr_correct,addrB_def]) >> fs [] >>
+       Cases_on `enable_stg 2 (agp32 fext fbits t)` >-
+       (subgoal `I' (2,SUC t) = I' (1,t)` >-
+         (fs [is_sch_def,is_sch_decode_def,Abbr `s`] >>
+          METIS_TAC []) >> fs [] >>
+        subgoal `I' (5,SUC t) = I' (4,t)` >-
+         (fs [is_sch_def,is_sch_writeback_def,is_sch_disable_def,Abbr `s`] >>
+          Cases_on `enable_stg 5 (agp32 fext fbits t)` >>
+          METIS_TAC []) >> fs [] >>
+        subgoal `I' (4,SUC t) = I' (3,t)` >-
+         (fs [is_sch_def,is_sch_memory_def,Abbr `s`] >>
+          `enable_stg 4 (agp32 fext fbits t)`
+            by fs [enable_stg_def,agp32_ID_ID_write_enable_MEM_state_flag] >>
+          Cases_on `isMemOp_hw_op (agp32 fext fbits t)` >>
+          fs [enable_stg_def] >>
+          METIS_TAC [MEM_stg_op_agp32_ID_EX_write_disable,
+                     agp32_ID_ID_write_enable_and_ID_EX_write_enable]) >> fs [] >>
+        subgoal `I' (3,SUC t) = I' (2,t)` >-
+         (fs [is_sch_def,is_sch_execute_def,Abbr `s`] >>
+          `enable_stg 3 (agp32 fext fbits t)`
+            by fs [enable_stg_def,agp32_ID_ID_write_enable_and_ID_EX_write_enable] >>
+          Cases_on `isJump_isa_op (I' (3,t)) a` >-
+           METIS_TAC [isJump_isa_op_not_none] >>
+          Cases_on `~reg_data_hazard (agp32 fext fbits t)` >>
+          METIS_TAC []) >> fs [] >>
+        `THE (I' (2,t)) = THE (I' (5,t)) + 1`
+          by METIS_TAC [EX_MEM_NONE_ID_instr_index_with_WB_instr_plus_1] >>
+        `THE (I' (5,t)) = THE (I' (2,t)) - 1` by fs [] >>
+        `THE (I' (1,t)) = THE (I' (2,t)) + 1`
+          by METIS_TAC [IF_instr_index_with_ID_instr_plus_1] >> fs [] >>
+        METIS_TAC [reg_adr_update_isa_not_change_data]) >>
+      `I' (2,SUC t) = I' (2,t)` by fs [is_sch_def,is_sch_disable_def] >>
+      subgoal `I' (5,SUC t) = I' (4,t)` >-
+       (fs [is_sch_def,is_sch_writeback_def,is_sch_disable_def,Abbr `s`] >>
+        Cases_on `enable_stg 5 (agp32 fext fbits t)` >>
+        METIS_TAC []) >> fs [] >>
+      Cases_on `enable_stg 3 (agp32 fext fbits t)` >-
+       (subgoal `I' (4,SUC t) = I' (3,t)` >-
+         (fs [is_sch_def,is_sch_memory_def,Abbr `s`] >>
+          `enable_stg 4 (agp32 fext fbits t)`
+            by fs [enable_stg_def,agp32_MEM_state_flag_eq_WB_state_flag] >>
+          Cases_on `isMemOp_hw_op (agp32 fext fbits t)` >>
+          fs [enable_stg_def] >>
+          METIS_TAC [MEM_stg_op_agp32_ID_EX_write_disable,enable_stg_def]) >> fs [] >>
+        `THE (I' (2,t)) = THE (I' (5,t)) + 1`
+          by METIS_TAC [EX_MEM_NONE_ID_instr_index_with_WB_instr_plus_1] >> fs []) >>
+      `I' (3,SUC t) = I' (3,t)` by METIS_TAC [is_sch_def,is_sch_disable_def] >> fs [] >>
+      `THE (I' (3,t)) = THE (I' (5,t)) + 1`
+        by METIS_TAC [EX_instr_index_with_WB_instr_plus_1_MEM_NONE] >>
+      `THE (I' (5,t)) = THE (I' (3,t)) - 1` by fs [] >>
+      `THE (I' (2,t)) = THE (I' (3,t)) + 1`
+        by METIS_TAC [ID_instr_index_with_EX_instr_plus_1] >> fs [] >>
+      METIS_TAC [reg_adr_update_isa_not_change_data]) >>
+    `~enable_stg 5 (agp32 fext fbits t)` by fs [enable_stg_def] >>
+    `I' (5,SUC t) = I' (5,t)` by METIS_TAC [is_sch_def,is_sch_disable_def] >> fs []) >-
    (** I (4,SUC t) and I (5,t) are not NONE **)
-   (`s.WB.WB_state_flag` by fs [Abbr `s`,enable_stg_def,agp32_ID_ID_write_enable_WB_state_flag] >>
-    `wb_data_vaild s` by fs [Abbr `s`,wb_data_vaild_def] >>
-    `(agp32 fext fbits (SUC t)).R = (FUNPOW Next (THE (I' (5,t))) a).R` by cheat >> fs [] >>
-    `(agp32 fext fbits (SUC t)).ID.ID_addrB = (15 >< 10) i`
-      by (fs [Abbr `i`,Abbr `s`,is_sch_def] >>
-          METIS_TAC [agp32_Rel_ag32_ID_addr_correct,addrB_def]) >> fs [] >>
-    subgoal `THE (I' (4,SUC t)) = THE (I' (5,t)) + 1` >-
-     (`I' (5,SUC t) = I' (4,t)`
+   (Cases_on`s.WB.WB_state_flag` >-
+     (`wb_data_vaild s` by fs [Abbr `s`,wb_data_vaild_def] >>
+      `(agp32 fext fbits (SUC t)).R = (FUNPOW Next (THE (I' (5,t))) a).R` by cheat >> fs [] >>
+      `(agp32 fext fbits (SUC t)).ID.ID_addrB = (15 >< 10) i`
+        by (fs [Abbr `i`,Abbr `s`,is_sch_def] >>
+            METIS_TAC [agp32_Rel_ag32_ID_addr_correct,addrB_def]) >> fs [] >>
+      Cases_on `enable_stg 2 (agp32 fext fbits t)` >-
+       (subgoal `THE (I' (4,SUC t)) = THE (I' (5,t)) + 1` >-
+         (`I' (5,SUC t) = I' (4,t)`
+            by (fs [is_sch_def,is_sch_writeback_def,is_sch_disable_def,Abbr `s`] >>
+                Cases_on `enable_stg 5 (agp32 fext fbits t)` >>
+                METIS_TAC []) >>
+          `I' (4,SUC t) = I' (3,t)`
+            by (fs [is_sch_def,is_sch_memory_def,Abbr `s`] >>
+                `enable_stg 4 (agp32 fext fbits t)`
+                  by fs [enable_stg_def,agp32_ID_ID_write_enable_MEM_state_flag] >>
+                Cases_on `isMemOp_hw_op (agp32 fext fbits t)` >>
+                fs [enable_stg_def] >>
+                METIS_TAC [MEM_stg_op_agp32_ID_EX_write_disable,
+                           agp32_ID_ID_write_enable_and_ID_EX_write_enable]) >> fs [] >>
+          METIS_TAC [EX_instr_index_with_WB_instr_plus_1_MEM_NONE]) >>
+        `THE (I' (5,t)) = THE (I' (4,SUC t)) - 1` by fs [] >> fs [] >>
+        `(FUNPOW Next (THE (I' (4,SUC t)) − 1) a).R ((15 >< 10) i) =
+        (FUNPOW Next (THE (I' (4,SUC t))) a).R ((15 >< 10) i)`
+          by METIS_TAC [reg_adr_update_isa_not_change_data] >> fs [] >>
+        `THE (I' (2,SUC t)) = THE (I' (4,SUC t)) + 1`
+          by METIS_TAC [EX_NONE_ID_instr_index_with_MEM_instr_plus_1] >> fs []) >>
+      `I' (2,SUC t) = I' (2,t)` by fs [is_sch_def,is_sch_disable_def] >>
+      subgoal `I' (4,SUC t) = I' (3,t)` >-
+       (fs [is_sch_def,is_sch_memory_def] >>
+        `enable_stg 4 (agp32 fext fbits t)`
+          by fs [enable_stg_def,agp32_MEM_state_flag_eq_WB_state_flag] >>
+        Cases_on `isMemOp_hw_op (agp32 fext fbits t)` >- METIS_TAC [] >> fs []) >>
+      `I' (5,SUC t) = I' (4,t)`
         by (fs [is_sch_def,is_sch_writeback_def,is_sch_disable_def,Abbr `s`] >>
             Cases_on `enable_stg 5 (agp32 fext fbits t)` >>
-            METIS_TAC []) >>
-      `I' (4,SUC t) = I' (3,t)`
-          by (fs [is_sch_def,is_sch_memory_def,Abbr `s`] >>
-              `enable_stg 4 (agp32 fext fbits t)`
-                by fs [enable_stg_def,agp32_ID_ID_write_enable_MEM_state_flag] >>
-              Cases_on `isMemOp_hw_op (agp32 fext fbits t)` >>
-              fs [enable_stg_def] >>
-              METIS_TAC [MEM_stg_op_agp32_ID_EX_write_disable,
-                         agp32_ID_ID_write_enable_and_ID_EX_write_enable]) >> fs [] >>
-      METIS_TAC [EX_instr_index_with_WB_instr_plus_1_MEM_NONE]) >>
-    `THE (I' (5,t)) = THE (I' (4,SUC t)) - 1` by fs [] >> fs [] >>
-    `(FUNPOW Next (THE (I' (4,SUC t)) − 1) a).R ((15 >< 10) i) =
-    (FUNPOW Next (THE (I' (4,SUC t))) a).R ((15 >< 10) i)`
-      by METIS_TAC [reg_adr_update_isa_not_change_data] >> fs [] >>
-    `THE (I' (2,SUC t)) = THE (I' (4,SUC t)) + 1`
-      by METIS_TAC [EX_NONE_ID_instr_index_with_MEM_instr_plus_1] >> fs []) >-
+            METIS_TAC []) >> fs [] >>
+      `THE (I' (3,t)) = THE (I' (5,t)) + 1`
+        by METIS_TAC [EX_instr_index_with_WB_instr_plus_1_MEM_NONE] >>
+      `THE (I' (5,t)) = THE (I' (3,t)) - 1` by fs [] >>
+      `THE (I' (2,t)) = THE (I' (3,t)) + 1`
+        by METIS_TAC [ID_instr_index_with_EX_instr_plus_1] >> fs [] >>
+      METIS_TAC [reg_adr_update_isa_not_change_data]) >>
+    `~enable_stg 5 (agp32 fext fbits t)` by fs [enable_stg_def] >>
+    `I' (5,SUC t) = I' (5,t)` by METIS_TAC [is_sch_def,is_sch_disable_def] >> fs []) >-
    (** I (3,SUC t), I (4,SUC t) and I (5,t) are not NONE **)
-   (`s.WB.WB_state_flag` by fs [Abbr `s`,enable_stg_def,agp32_ID_ID_write_enable_WB_state_flag] >>
-    `wb_data_vaild s` by fs [Abbr `s`,wb_data_vaild_def] >>
+   (Cases_on `s.WB.WB_state_flag` >-
+     (`wb_data_vaild s` by fs [Abbr `s`,wb_data_vaild_def] >>
+      `(agp32 fext fbits (SUC t)).R = (FUNPOW Next (THE (I' (5,t))) a).R` by cheat >> fs [] >>
+      `(agp32 fext fbits (SUC t)).ID.ID_addrB = (15 >< 10) i`
+        by (fs [Abbr `i`,Abbr `s`,is_sch_def] >>
+            METIS_TAC [agp32_Rel_ag32_ID_addr_correct,addrB_def]) >> fs [] >>
+      Cases_on `enable_stg 2 (agp32 fext fbits t)` >-
+       (subgoal `THE (I' (4,SUC t)) = THE (I' (5,t)) + 1` >-
+         (`I' (5,SUC t) = I' (4,t)`
+            by (fs [is_sch_def,is_sch_writeback_def,is_sch_disable_def,Abbr `s`] >>
+                Cases_on `enable_stg 5 (agp32 fext fbits t)` >>
+                METIS_TAC []) >>
+          `I' (4,SUC t) = I' (3,t)`
+            by (fs [is_sch_def,is_sch_memory_def,Abbr `s`] >>
+                `enable_stg 4 (agp32 fext fbits t)`
+                  by fs [enable_stg_def,agp32_ID_ID_write_enable_MEM_state_flag] >>
+                Cases_on `isMemOp_hw_op (agp32 fext fbits t)` >>
+                fs [enable_stg_def] >>
+                METIS_TAC [MEM_stg_op_agp32_ID_EX_write_disable,
+                           agp32_ID_ID_write_enable_and_ID_EX_write_enable]) >> fs [] >>
+          METIS_TAC [EX_instr_index_with_WB_instr_plus_1_MEM_NONE]) >>
+        `THE (I' (5,t)) = THE (I' (4,SUC t)) - 1` by fs [] >> fs [] >>
+        `(FUNPOW Next (THE (I' (4,SUC t)) − 1) a).R ((15 >< 10) i) =
+        (FUNPOW Next (THE (I' (4,SUC t))) a).R ((15 >< 10) i)`
+          by METIS_TAC [reg_adr_update_isa_not_change_data] >> fs [] >>
+        `THE (I' (3,SUC t)) = THE (I' (4,SUC t)) + 1`
+          by METIS_TAC [EX_instr_index_with_MEM_instr_plus_1] >>
+        `THE (I' (2,SUC t)) = THE (I' (3,SUC t)) + 1`
+          by METIS_TAC [ID_instr_index_with_EX_instr_plus_1] >> fs [] >>
+        `THE (I' (4,SUC t)) = THE (I' (3,SUC t)) - 1` by FULL_SIMP_TAC std_ss [] >>
+        METIS_TAC [reg_adr_update_isa_not_change_data]) >>
+      `I' (2,SUC t) = I' (2,t)` by fs [is_sch_def,is_sch_disable_def] >>
+      subgoal `I' (4,SUC t) = I' (3,t)` >-
+       (fs [is_sch_def,is_sch_memory_def] >>
+        `enable_stg 4 (agp32 fext fbits t)`
+          by fs [enable_stg_def,agp32_MEM_state_flag_eq_WB_state_flag] >>
+        Cases_on `isMemOp_hw_op (agp32 fext fbits t)` >- METIS_TAC [] >> fs []) >>
+      `I' (5,SUC t) = I' (4,t)`
+        by (fs [is_sch_def,is_sch_writeback_def,is_sch_disable_def,Abbr `s`] >>
+            Cases_on `enable_stg 5 (agp32 fext fbits t)` >>
+            METIS_TAC []) >> fs [] >>
+      `THE (I' (3,t)) = THE (I' (5,t)) + 1`
+        by METIS_TAC [EX_instr_index_with_WB_instr_plus_1_MEM_NONE] >>
+      `THE (I' (5,t)) = THE (I' (3,t)) - 1` by fs [] >>
+      `THE (I' (2,t)) = THE (I' (3,t)) + 1`
+        by METIS_TAC [ID_instr_index_with_EX_instr_plus_1] >> fs [] >>
+      METIS_TAC [reg_adr_update_isa_not_change_data]) >>
+    `~enable_stg 5 (agp32 fext fbits t)` by fs [enable_stg_def] >>
+    `I' (5,SUC t) = I' (5,t)` by METIS_TAC [is_sch_def,is_sch_disable_def] >> fs []) >-
+   (** I (5,SUC t) and I (5,t) are not NONE **)
+   (Cases_on `s.WB.WB_state_flag` >-
+     (`wb_data_vaild s` by fs [Abbr `s`,wb_data_vaild_def] >>
+      `(agp32 fext fbits (SUC t)).R = (FUNPOW Next (THE (I' (5,t))) a).R` by cheat >> fs [] >>
+      `(agp32 fext fbits (SUC t)).ID.ID_addrB = (15 >< 10) i`
+        by (fs [Abbr `i`,Abbr `s`,is_sch_def] >>
+            METIS_TAC [agp32_Rel_ag32_ID_addr_correct,addrB_def]) >> fs [] >>
+      `enable_stg 5 (agp32 fext fbits t)`
+        by fs [enable_stg_def,agp32_ID_ID_write_enable_WB_state_flag] >>
+      `THE (I' (5,SUC t)) = THE (I' (5,t)) + 1` by METIS_TAC [WB_instr_index_t_SUC_t_enable] >>
+      `THE (I' (5,t)) = THE (I' (5,SUC t)) - 1` by fs [] >> fs [] >>
+      `(FUNPOW Next (THE (I' (5,SUC t)) − 1) a).R ((15 >< 10) i) =
+      (FUNPOW Next (THE (I' (5,SUC t))) a).R ((15 >< 10) i)`
+        by METIS_TAC [reg_adr_update_isa_not_change_data] >> fs [] >>
+      `THE (I' (2,SUC t)) = THE (I' (5,SUC t)) + 1`
+        by METIS_TAC [EX_MEM_NONE_ID_instr_index_with_WB_instr_plus_1] >> fs []) >>
+    `~enable_stg 5 (agp32 fext fbits t)` by fs [enable_stg_def] >>
+    `~enable_stg 4 (agp32 fext fbits t)`
+      by fs [enable_stg_def,agp32_MEM_state_flag_eq_WB_state_flag] >>
+    `~(agp32 fext fbits t).ID.ID_ID_write_enable /\ ~(agp32 fext fbits t).ID.ID_EX_write_enable`
+      by METIS_TAC [agp32_ID_EX_write_enable_WB_state_flag,agp32_ID_ID_write_enable_WB_state_flag] >>
+    `~enable_stg 2 (agp32 fext fbits t) /\
+    ~enable_stg 3 (agp32 fext fbits t)` by fs [enable_stg_def] >>
+    `(agp32 fext fbits (SUC t)).ID.ID_addrB = s.ID.ID_addrB`
+      by METIS_TAC [Abbr `s`,is_sch_def,agp32_ID_disabled_ID_addr_unchanged] >>
+    `(agp32 fext fbits (SUC t)).ID.ID_addrB_disable = (agp32 fext fbits t).ID.ID_addrB_disable`
+      by METIS_TAC [Abbr `s`,is_sch_def,agp32_ID_disabled_ID_flag_unchanged] >>
+    `(agp32 fext fbits (SUC t)).ID.ID_read_dataB = (agp32 fext fbits t).ID.ID_read_dataB`
+      by METIS_TAC [Abbr `s`,is_sch_def,agp32_ID_disabled_ID_read_data_unchanged] >>
+    `(I' (2,SUC t) = I' (2,t)) /\ (I' (3,SUC t) = I' (3,t)) /\
+    (I' (4,SUC t) = I' (4,t)) /\ (I' (5,SUC t) = I' (5,t))` by METIS_TAC [is_sch_def,is_sch_disable_def] >>
+    fs [Rel_def,ID_reg_data_Rel_def,reg_dataB_def,addrB_def] >> METIS_TAC []) >-
+   (** I (3,SUC t), I (5,SUC t) and I (5,t) are not NONE **)
+   (Cases_on `s.WB.WB_state_flag` >-
+     (`wb_data_vaild s` by fs [Abbr `s`,wb_data_vaild_def] >>
+      `(agp32 fext fbits (SUC t)).R = (FUNPOW Next (THE (I' (5,t))) a).R` by cheat >> fs [] >>
+      `(agp32 fext fbits (SUC t)).ID.ID_addrB = (15 >< 10) i`
+        by (fs [Abbr `i`,Abbr `s`,is_sch_def] >>
+            METIS_TAC [agp32_Rel_ag32_ID_addr_correct,addrB_def]) >> fs [] >>
+      `enable_stg 5 (agp32 fext fbits t)`
+        by fs [enable_stg_def,agp32_ID_ID_write_enable_WB_state_flag] >>
+      `THE (I' (5,SUC t)) = THE (I' (5,t)) + 1` by METIS_TAC [WB_instr_index_t_SUC_t_enable] >>
+      `THE (I' (5,t)) = THE (I' (5,SUC t)) - 1` by fs [] >> fs [] >>
+      `(FUNPOW Next (THE (I' (5,SUC t)) − 1) a).R ((15 >< 10) i) =
+      (FUNPOW Next (THE (I' (5,SUC t))) a).R ((15 >< 10) i)`
+        by METIS_TAC [reg_adr_update_isa_not_change_data] >> fs [] >>
+      `THE (I' (3,SUC t)) = THE (I' (5,SUC t)) + 1`
+        by METIS_TAC [EX_instr_index_with_WB_instr_plus_1_MEM_NONE] >>
+      `THE (I' (2,SUC t)) = THE (I' (3,SUC t)) + 1`
+        by METIS_TAC [ID_instr_index_with_EX_instr_plus_1] >> fs [] >>
+      `THE (I' (5,SUC t)) = THE (I' (3,SUC t)) - 1` by fs [] >>
+      METIS_TAC [reg_adr_update_isa_not_change_data]) >>
+    `~enable_stg 5 (agp32 fext fbits t)` by fs [enable_stg_def] >>
+    `~enable_stg 4 (agp32 fext fbits t)`
+      by fs [enable_stg_def,agp32_MEM_state_flag_eq_WB_state_flag] >>
+    `~(agp32 fext fbits t).ID.ID_ID_write_enable /\ ~(agp32 fext fbits t).ID.ID_EX_write_enable`
+      by METIS_TAC [agp32_ID_EX_write_enable_WB_state_flag,agp32_ID_ID_write_enable_WB_state_flag] >>
+    `~enable_stg 2 (agp32 fext fbits t) /\
+    ~enable_stg 3 (agp32 fext fbits t)` by fs [enable_stg_def] >>
+    `(agp32 fext fbits (SUC t)).ID.ID_addrB = s.ID.ID_addrB`
+      by METIS_TAC [Abbr `s`,is_sch_def,agp32_ID_disabled_ID_addr_unchanged] >>
+    `(agp32 fext fbits (SUC t)).ID.ID_addrB_disable = (agp32 fext fbits t).ID.ID_addrB_disable`
+      by METIS_TAC [Abbr `s`,is_sch_def,agp32_ID_disabled_ID_flag_unchanged] >>
+    `(agp32 fext fbits (SUC t)).ID.ID_read_dataB = (agp32 fext fbits t).ID.ID_read_dataB`
+      by METIS_TAC [Abbr `s`,is_sch_def,agp32_ID_disabled_ID_read_data_unchanged] >>
+    `(I' (2,SUC t) = I' (2,t)) /\ (I' (3,SUC t) = I' (3,t)) /\
+    (I' (4,SUC t) = I' (4,t)) /\ (I' (5,SUC t) = I' (5,t))` by METIS_TAC [is_sch_def,is_sch_disable_def] >>
+    fs [Rel_def,ID_reg_data_Rel_def,reg_dataB_def,addrB_def] >> METIS_TAC []) >-
+   (** I (4,SUC t), I (5,SUC t) and I (5,t) are not NONE **)
+   (Cases_on `s.WB.WB_state_flag` >-
+     (`wb_data_vaild s` by fs [Abbr `s`,wb_data_vaild_def] >>
+      `(agp32 fext fbits (SUC t)).R = (FUNPOW Next (THE (I' (5,t))) a).R` by cheat >> fs [] >>
+      `(agp32 fext fbits (SUC t)).ID.ID_addrB = (15 >< 10) i`
+        by (fs [Abbr `i`,Abbr `s`,is_sch_def] >>
+            METIS_TAC [agp32_Rel_ag32_ID_addr_correct,addrB_def]) >> fs [] >>
+      `enable_stg 5 (agp32 fext fbits t)`
+        by fs [enable_stg_def,agp32_ID_ID_write_enable_WB_state_flag] >>
+      `THE (I' (5,SUC t)) = THE (I' (5,t)) + 1` by METIS_TAC [WB_instr_index_t_SUC_t_enable] >>
+      `THE (I' (5,t)) = THE (I' (5,SUC t)) - 1` by fs [] >> fs [] >>
+      `(FUNPOW Next (THE (I' (5,SUC t)) − 1) a).R ((15 >< 10) i) =
+      (FUNPOW Next (THE (I' (5,SUC t))) a).R ((15 >< 10) i)`
+        by METIS_TAC [reg_adr_update_isa_not_change_data] >> fs [] >>
+      `THE (I' (4,SUC t)) = THE (I' (5,SUC t)) + 1`
+        by METIS_TAC [MEM_instr_index_with_WB_instr_plus_1] >>
+      `THE (I' (2,SUC t)) = THE (I' (4,SUC t)) + 1`
+        by METIS_TAC [EX_NONE_ID_instr_index_with_MEM_instr_plus_1] >> fs [] >>
+      `THE (I' (5,SUC t)) = THE (I' (4,SUC t)) - 1` by fs [] >>
+      METIS_TAC [reg_adr_update_isa_not_change_data]) >>
+    `~enable_stg 5 (agp32 fext fbits t)` by fs [enable_stg_def] >>
+    `~enable_stg 4 (agp32 fext fbits t)`
+      by fs [enable_stg_def,agp32_MEM_state_flag_eq_WB_state_flag] >>
+    `~(agp32 fext fbits t).ID.ID_ID_write_enable /\ ~(agp32 fext fbits t).ID.ID_EX_write_enable`
+      by METIS_TAC [agp32_ID_EX_write_enable_WB_state_flag,agp32_ID_ID_write_enable_WB_state_flag] >>
+    `~enable_stg 2 (agp32 fext fbits t) /\
+    ~enable_stg 3 (agp32 fext fbits t)` by fs [enable_stg_def] >>
+    `(agp32 fext fbits (SUC t)).ID.ID_addrB = s.ID.ID_addrB`
+      by METIS_TAC [Abbr `s`,is_sch_def,agp32_ID_disabled_ID_addr_unchanged] >>
+    `(agp32 fext fbits (SUC t)).ID.ID_addrB_disable = (agp32 fext fbits t).ID.ID_addrB_disable`
+      by METIS_TAC [Abbr `s`,is_sch_def,agp32_ID_disabled_ID_flag_unchanged] >>
+    `(agp32 fext fbits (SUC t)).ID.ID_read_dataB = (agp32 fext fbits t).ID.ID_read_dataB`
+      by METIS_TAC [Abbr `s`,is_sch_def,agp32_ID_disabled_ID_read_data_unchanged] >>
+    `(I' (2,SUC t) = I' (2,t)) /\ (I' (3,SUC t) = I' (3,t)) /\
+    (I' (4,SUC t) = I' (4,t)) /\ (I' (5,SUC t) = I' (5,t))` by METIS_TAC [is_sch_def,is_sch_disable_def] >>
+    fs [Rel_def,ID_reg_data_Rel_def,reg_dataB_def,addrB_def] >> METIS_TAC []) >>
+  (** all are not NONE **)
+  Cases_on `s.WB.WB_state_flag` >-
+   (`wb_data_vaild s` by fs [Abbr `s`,wb_data_vaild_def] >>
     `(agp32 fext fbits (SUC t)).R = (FUNPOW Next (THE (I' (5,t))) a).R` by cheat >> fs [] >>
     `(agp32 fext fbits (SUC t)).ID.ID_addrB = (15 >< 10) i`
       by (fs [Abbr `i`,Abbr `s`,is_sch_def] >>
           METIS_TAC [agp32_Rel_ag32_ID_addr_correct,addrB_def]) >> fs [] >>
-    subgoal `THE (I' (4,SUC t)) = THE (I' (5,t)) + 1` >-
-     (`I' (5,SUC t) = I' (4,t)`
-        by (fs [is_sch_def,is_sch_writeback_def,is_sch_disable_def,Abbr `s`] >>
-            Cases_on `enable_stg 5 (agp32 fext fbits t)` >>
-            METIS_TAC []) >>
-      `I' (4,SUC t) = I' (3,t)`
-          by (fs [is_sch_def,is_sch_memory_def,Abbr `s`] >>
-              `enable_stg 4 (agp32 fext fbits t)`
-                by fs [enable_stg_def,agp32_ID_ID_write_enable_MEM_state_flag] >>
-              Cases_on `isMemOp_hw_op (agp32 fext fbits t)` >>
-              fs [enable_stg_def] >>
-              METIS_TAC [MEM_stg_op_agp32_ID_EX_write_disable,
-                         agp32_ID_ID_write_enable_and_ID_EX_write_enable]) >> fs [] >>
-      METIS_TAC [EX_instr_index_with_WB_instr_plus_1_MEM_NONE]) >>
-    `THE (I' (5,t)) = THE (I' (4,SUC t)) - 1` by fs [] >> fs [] >>
+    `enable_stg 5 (agp32 fext fbits t)`
+      by fs [enable_stg_def,agp32_ID_ID_write_enable_WB_state_flag] >>
+    `THE (I' (5,SUC t)) = THE (I' (5,t)) + 1` by METIS_TAC [WB_instr_index_t_SUC_t_enable] >>
+    `THE (I' (5,t)) = THE (I' (5,SUC t)) - 1` by fs [] >> fs [] >>
+    `(FUNPOW Next (THE (I' (5,SUC t)) − 1) a).R ((15 >< 10) i) =
+    (FUNPOW Next (THE (I' (5,SUC t))) a).R ((15 >< 10) i)`
+      by METIS_TAC [reg_adr_update_isa_not_change_data] >> fs [] >>
+    qpat_x_assum `THE (I' (5,SUC t)) = _` (fn thm => all_tac)  >>
+    `THE (I' (4,SUC t)) = THE (I' (5,SUC t)) + 1`
+      by METIS_TAC [MEM_instr_index_with_WB_instr_plus_1] >>
+    `THE (I' (5,SUC t)) = THE (I' (4,SUC t)) - 1` by fs [] >> fs [] >>
     `(FUNPOW Next (THE (I' (4,SUC t)) − 1) a).R ((15 >< 10) i) =
     (FUNPOW Next (THE (I' (4,SUC t))) a).R ((15 >< 10) i)`
       by METIS_TAC [reg_adr_update_isa_not_change_data] >> fs [] >>
@@ -1281,90 +1705,23 @@ Proof
     `THE (I' (2,SUC t)) = THE (I' (3,SUC t)) + 1`
       by METIS_TAC [ID_instr_index_with_EX_instr_plus_1] >> fs [] >>
     `THE (I' (4,SUC t)) = THE (I' (3,SUC t)) - 1` by FULL_SIMP_TAC std_ss [] >>
-    METIS_TAC [reg_adr_update_isa_not_change_data]) >-
-   (** I (5,SUC t) and I (5,t) are not NONE **)
-   (`s.WB.WB_state_flag` by fs [Abbr `s`,enable_stg_def,agp32_ID_ID_write_enable_WB_state_flag] >>
-    `wb_data_vaild s` by fs [Abbr `s`,wb_data_vaild_def] >>
-    `(agp32 fext fbits (SUC t)).R = (FUNPOW Next (THE (I' (5,t))) a).R` by cheat >> fs [] >>
-    `(agp32 fext fbits (SUC t)).ID.ID_addrB = (15 >< 10) i`
-      by (fs [Abbr `i`,Abbr `s`,is_sch_def] >>
-          METIS_TAC [agp32_Rel_ag32_ID_addr_correct,addrB_def]) >> fs [] >>
-    `enable_stg 5 (agp32 fext fbits t)`
-      by fs [enable_stg_def,agp32_ID_ID_write_enable_WB_state_flag] >>
-    `THE (I' (5,SUC t)) = THE (I' (5,t)) + 1` by METIS_TAC [WB_instr_index_t_SUC_t_enable] >>
-    `THE (I' (5,t)) = THE (I' (5,SUC t)) - 1` by fs [] >> fs [] >>
-    `(FUNPOW Next (THE (I' (5,SUC t)) − 1) a).R ((15 >< 10) i) =
-    (FUNPOW Next (THE (I' (5,SUC t))) a).R ((15 >< 10) i)`
-      by METIS_TAC [reg_adr_update_isa_not_change_data] >> fs [] >>
-    `THE (I' (2,SUC t)) = THE (I' (5,SUC t)) + 1`
-      by METIS_TAC [EX_MEM_NONE_ID_instr_index_with_WB_instr_plus_1] >> fs []) >-
-   (** I (3,SUC t), I (5,SUC t) and I (5,t) are not NONE **)
-   (`s.WB.WB_state_flag` by fs [Abbr `s`,enable_stg_def,agp32_ID_ID_write_enable_WB_state_flag] >>
-    `wb_data_vaild s` by fs [Abbr `s`,wb_data_vaild_def] >>
-    `(agp32 fext fbits (SUC t)).R = (FUNPOW Next (THE (I' (5,t))) a).R` by cheat >> fs [] >>
-    `(agp32 fext fbits (SUC t)).ID.ID_addrB = (15 >< 10) i`
-      by (fs [Abbr `i`,Abbr `s`,is_sch_def] >>
-          METIS_TAC [agp32_Rel_ag32_ID_addr_correct,addrB_def]) >> fs [] >>
-    `enable_stg 5 (agp32 fext fbits t)`
-      by fs [enable_stg_def,agp32_ID_ID_write_enable_WB_state_flag] >>
-    `THE (I' (5,SUC t)) = THE (I' (5,t)) + 1` by METIS_TAC [WB_instr_index_t_SUC_t_enable] >>
-    `THE (I' (5,t)) = THE (I' (5,SUC t)) - 1` by fs [] >> fs [] >>
-    `(FUNPOW Next (THE (I' (5,SUC t)) − 1) a).R ((15 >< 10) i) =
-    (FUNPOW Next (THE (I' (5,SUC t))) a).R ((15 >< 10) i)`
-      by METIS_TAC [reg_adr_update_isa_not_change_data] >> fs [] >>
-    `THE (I' (3,SUC t)) = THE (I' (5,SUC t)) + 1`
-      by METIS_TAC [EX_instr_index_with_WB_instr_plus_1_MEM_NONE] >>
-    `THE (I' (2,SUC t)) = THE (I' (3,SUC t)) + 1`
-      by METIS_TAC [ID_instr_index_with_EX_instr_plus_1] >> fs [] >>
-    `THE (I' (5,SUC t)) = THE (I' (3,SUC t)) - 1` by fs [] >>
-    METIS_TAC [reg_adr_update_isa_not_change_data]) >-
-   (** I (4,SUC t), I (5,SUC t) and I (5,t) are not NONE **)
-   (`s.WB.WB_state_flag` by fs [Abbr `s`,enable_stg_def,agp32_ID_ID_write_enable_WB_state_flag] >>
-    `wb_data_vaild s` by fs [Abbr `s`,wb_data_vaild_def] >>
-    `(agp32 fext fbits (SUC t)).R = (FUNPOW Next (THE (I' (5,t))) a).R` by cheat >> fs [] >>
-    `(agp32 fext fbits (SUC t)).ID.ID_addrB = (15 >< 10) i`
-      by (fs [Abbr `i`,Abbr `s`,is_sch_def] >>
-          METIS_TAC [agp32_Rel_ag32_ID_addr_correct,addrB_def]) >> fs [] >>
-    `enable_stg 5 (agp32 fext fbits t)`
-      by fs [enable_stg_def,agp32_ID_ID_write_enable_WB_state_flag] >>
-    `THE (I' (5,SUC t)) = THE (I' (5,t)) + 1` by METIS_TAC [WB_instr_index_t_SUC_t_enable] >>
-    `THE (I' (5,t)) = THE (I' (5,SUC t)) - 1` by fs [] >> fs [] >>
-    `(FUNPOW Next (THE (I' (5,SUC t)) − 1) a).R ((15 >< 10) i) =
-    (FUNPOW Next (THE (I' (5,SUC t))) a).R ((15 >< 10) i)`
-      by METIS_TAC [reg_adr_update_isa_not_change_data] >> fs [] >>
-    `THE (I' (4,SUC t)) = THE (I' (5,SUC t)) + 1`
-      by METIS_TAC [MEM_instr_index_with_WB_instr_plus_1] >>
-    `THE (I' (2,SUC t)) = THE (I' (4,SUC t)) + 1`
-      by METIS_TAC [EX_NONE_ID_instr_index_with_MEM_instr_plus_1] >> fs [] >>
-    `THE (I' (5,SUC t)) = THE (I' (4,SUC t)) - 1` by fs [] >>
     METIS_TAC [reg_adr_update_isa_not_change_data]) >>
-  (** all are not NONE **)
-  `s.WB.WB_state_flag` by fs [Abbr `s`,enable_stg_def,agp32_ID_ID_write_enable_WB_state_flag] >>
-  `wb_data_vaild s` by fs [Abbr `s`,wb_data_vaild_def] >>
-  `(agp32 fext fbits (SUC t)).R = (FUNPOW Next (THE (I' (5,t))) a).R` by cheat >> fs [] >>
-  `(agp32 fext fbits (SUC t)).ID.ID_addrB = (15 >< 10) i`
-    by (fs [Abbr `i`,Abbr `s`,is_sch_def] >>
-        METIS_TAC [agp32_Rel_ag32_ID_addr_correct,addrB_def]) >> fs [] >>
-  `enable_stg 5 (agp32 fext fbits t)`
-    by fs [enable_stg_def,agp32_ID_ID_write_enable_WB_state_flag] >>
-  `THE (I' (5,SUC t)) = THE (I' (5,t)) + 1` by METIS_TAC [WB_instr_index_t_SUC_t_enable] >>
-  `THE (I' (5,t)) = THE (I' (5,SUC t)) - 1` by fs [] >> fs [] >>
-  `(FUNPOW Next (THE (I' (5,SUC t)) − 1) a).R ((15 >< 10) i) =
-  (FUNPOW Next (THE (I' (5,SUC t))) a).R ((15 >< 10) i)`
-    by METIS_TAC [reg_adr_update_isa_not_change_data] >> fs [] >>
-  qpat_x_assum `THE (I' (5,SUC t)) = _` (fn thm => all_tac)  >>
-  `THE (I' (4,SUC t)) = THE (I' (5,SUC t)) + 1`
-    by METIS_TAC [MEM_instr_index_with_WB_instr_plus_1] >>
-  `THE (I' (5,SUC t)) = THE (I' (4,SUC t)) - 1` by fs [] >> fs [] >>
-  `(FUNPOW Next (THE (I' (4,SUC t)) − 1) a).R ((15 >< 10) i) =
-  (FUNPOW Next (THE (I' (4,SUC t))) a).R ((15 >< 10) i)`
-    by METIS_TAC [reg_adr_update_isa_not_change_data] >> fs [] >>
-  `THE (I' (3,SUC t)) = THE (I' (4,SUC t)) + 1`
-    by METIS_TAC [EX_instr_index_with_MEM_instr_plus_1] >>
-  `THE (I' (2,SUC t)) = THE (I' (3,SUC t)) + 1`
-    by METIS_TAC [ID_instr_index_with_EX_instr_plus_1] >> fs [] >>
-  `THE (I' (4,SUC t)) = THE (I' (3,SUC t)) - 1` by FULL_SIMP_TAC std_ss [] >>
-  METIS_TAC [reg_adr_update_isa_not_change_data]
+  `~enable_stg 5 (agp32 fext fbits t)` by fs [enable_stg_def] >>
+  `~enable_stg 4 (agp32 fext fbits t)`
+    by fs [enable_stg_def,agp32_MEM_state_flag_eq_WB_state_flag] >>
+  `~(agp32 fext fbits t).ID.ID_ID_write_enable /\ ~(agp32 fext fbits t).ID.ID_EX_write_enable`
+    by METIS_TAC [agp32_ID_EX_write_enable_WB_state_flag,agp32_ID_ID_write_enable_WB_state_flag] >>
+  `~enable_stg 2 (agp32 fext fbits t) /\
+  ~enable_stg 3 (agp32 fext fbits t)` by fs [enable_stg_def] >>
+  `(agp32 fext fbits (SUC t)).ID.ID_addrB = s.ID.ID_addrB`
+    by METIS_TAC [Abbr `s`,is_sch_def,agp32_ID_disabled_ID_addr_unchanged] >>
+  `(agp32 fext fbits (SUC t)).ID.ID_addrB_disable = (agp32 fext fbits t).ID.ID_addrB_disable`
+    by METIS_TAC [Abbr `s`,is_sch_def,agp32_ID_disabled_ID_flag_unchanged] >>
+  `(agp32 fext fbits (SUC t)).ID.ID_read_dataB = (agp32 fext fbits t).ID.ID_read_dataB`
+    by METIS_TAC [Abbr `s`,is_sch_def,agp32_ID_disabled_ID_read_data_unchanged] >>
+  `(I' (2,SUC t) = I' (2,t)) /\ (I' (3,SUC t) = I' (3,t)) /\
+  (I' (4,SUC t) = I' (4,t)) /\ (I' (5,SUC t) = I' (5,t))` by METIS_TAC [is_sch_def,is_sch_disable_def] >>
+  fs [Rel_def,ID_reg_data_Rel_def,reg_dataB_def,addrB_def] >> METIS_TAC []
 QED
 
 
@@ -1373,8 +1730,8 @@ Theorem agp32_Rel_ag32_ID_read_dataW_no_write_before:
   !fext fbits a t I.
     is_sch I (agp32 fext fbits) a ==>
     Rel I (fext t) (agp32 fext fbits (t-1)) (agp32 fext fbits t) a t ==>
-    enable_stg 2 (agp32 fext fbits t) ==>
     I (2,SUC t) <> NONE ==>
+    ~(agp32 fext fbits (SUC t)).ID.ID_addrW_disable ==>
     ~reg_adr_update_isa (I (3,SUC t)) a (agp32 fext fbits (SUC t)).ID.ID_addrW ==>
     ~reg_adr_update_isa (I (4,SUC t)) a (agp32 fext fbits (SUC t)).ID.ID_addrW ==>
     ~reg_adr_update_isa (I (5,SUC t)) a (agp32 fext fbits (SUC t)).ID.ID_addrW ==>
@@ -1500,123 +1857,336 @@ Proof
     `THE (I' (4,SUC t)) = THE (I' (3,SUC t)) - 1` by FULL_SIMP_TAC std_ss [] >>
     METIS_TAC [reg_adr_update_isa_not_change_data]) >-
    (** I (5,t) is not NONE **)
-   (`s.WB.WB_state_flag` by fs [Abbr `s`,enable_stg_def,agp32_ID_ID_write_enable_WB_state_flag] >>
-    `wb_data_vaild s` by fs [Abbr `s`,wb_data_vaild_def] >>
-    `(agp32 fext fbits (SUC t)).R = (FUNPOW Next (THE (I' (5,t))) a).R` by cheat >> fs [] >>
-    subgoal `I' (2,SUC t) = I' (1,t)` >-
-     (fs [is_sch_def,is_sch_decode_def,Abbr `s`] >>
-      Cases_on `isJump_isa_op (I' (2,t)) a \/ isJump_isa_op (I' (3,t)) a` >>
-      METIS_TAC []) >> fs [] >>
-    subgoal `I' (5,SUC t) = I' (4,t)` >-
-     (fs [is_sch_def,is_sch_writeback_def,is_sch_disable_def,Abbr `s`] >>
-      Cases_on `enable_stg 5 (agp32 fext fbits t)` >>
-      METIS_TAC []) >> fs [] >>
-    subgoal `I' (4,SUC t) = I' (3,t)` >-
-     (fs [is_sch_def,is_sch_memory_def,Abbr `s`] >>
-      `enable_stg 4 (agp32 fext fbits t)`
-        by fs [enable_stg_def,agp32_ID_ID_write_enable_MEM_state_flag] >>
-      Cases_on `isMemOp_hw_op (agp32 fext fbits t)` >>
-      fs [enable_stg_def] >>
-      METIS_TAC [MEM_stg_op_agp32_ID_EX_write_disable,
-                 agp32_ID_ID_write_enable_and_ID_EX_write_enable]) >> fs [] >>
-    subgoal `I' (3,SUC t) = I' (2,t)` >-
-     (fs [is_sch_def,is_sch_execute_def,Abbr `s`] >>
-      `enable_stg 3 (agp32 fext fbits t)`
-        by fs [enable_stg_def,agp32_ID_ID_write_enable_and_ID_EX_write_enable] >>
-      Cases_on `isJump_hw_op (agp32 fext fbits t)` >-
-       (`isJump_isa_op (I' (3,t)) a` by fs [isJump_hw_op_def,Rel_def,EX_Rel_spec_def] >>
-         METIS_TAC [isJump_isa_op_not_none]) >>
-      Cases_on `~reg_data_hazard (agp32 fext fbits t)` >- METIS_TAC [] >>
-      fs [isJump_hw_op_def,enable_stg_def] >>
-      METIS_TAC [agp32_ID_ID_write_enable_EX_jump_sel_then_no_reg_data_hazard]) >> fs [] >>
-    `THE (I' (1,t)) = THE (I' (5,t)) + 1`
-      by METIS_TAC [ID_EX_MEM_NONE_IF_instr_index_with_WB_instr_plus_1] >> fs []) >-
+   (Cases_on `s.WB.WB_state_flag` >-
+     (`wb_data_vaild s` by fs [Abbr `s`,wb_data_vaild_def] >>
+      `(agp32 fext fbits (SUC t)).R = (FUNPOW Next (THE (I' (5,t))) a).R` by cheat >> fs [] >>
+      Cases_on `enable_stg 2 (agp32 fext fbits t)` >-
+       (subgoal `I' (2,SUC t) = I' (1,t)` >-
+         (fs [is_sch_def,is_sch_decode_def,Abbr `s`] >>
+          METIS_TAC []) >> fs [] >>
+        subgoal `I' (5,SUC t) = I' (4,t)` >-
+         (fs [is_sch_def,is_sch_writeback_def,is_sch_disable_def,Abbr `s`] >>
+          Cases_on `enable_stg 5 (agp32 fext fbits t)` >>
+          METIS_TAC []) >> fs [] >>
+        subgoal `I' (4,SUC t) = I' (3,t)` >-
+         (fs [is_sch_def,is_sch_memory_def,Abbr `s`] >>
+          `enable_stg 4 (agp32 fext fbits t)`
+            by fs [enable_stg_def,agp32_ID_ID_write_enable_MEM_state_flag] >>
+          Cases_on `isMemOp_hw_op (agp32 fext fbits t)` >>
+          fs [enable_stg_def] >>
+          METIS_TAC [MEM_stg_op_agp32_ID_EX_write_disable,
+                     agp32_ID_ID_write_enable_and_ID_EX_write_enable]) >> fs [] >>
+        subgoal `I' (3,SUC t) = I' (2,t)` >-
+         (fs [is_sch_def,is_sch_execute_def,Abbr `s`] >>
+          `enable_stg 3 (agp32 fext fbits t)`
+            by fs [enable_stg_def,agp32_ID_ID_write_enable_and_ID_EX_write_enable] >>
+          Cases_on `isJump_hw_op (agp32 fext fbits t)` >-
+           (`isJump_isa_op (I' (3,t)) a` by fs [isJump_hw_op_def,Rel_def,EX_Rel_spec_def] >>
+            METIS_TAC [isJump_isa_op_not_none]) >>
+          Cases_on `~reg_data_hazard (agp32 fext fbits t)` >- METIS_TAC [] >>
+          fs [isJump_hw_op_def,enable_stg_def] >>
+          METIS_TAC [agp32_ID_ID_write_enable_EX_jump_sel_then_no_reg_data_hazard]) >> fs [] >>
+        `THE (I' (1,t)) = THE (I' (5,t)) + 1`
+          by METIS_TAC [ID_EX_MEM_NONE_IF_instr_index_with_WB_instr_plus_1] >> fs []) >>
+      `I' (2,SUC t) = I' (2,t)` by fs [is_sch_def,is_sch_disable_def] >>
+      subgoal `I' (5,SUC t) = I' (4,t)` >-
+       (fs [is_sch_def,is_sch_writeback_def,is_sch_disable_def,Abbr `s`] >>
+        Cases_on `enable_stg 5 (agp32 fext fbits t)` >>
+        METIS_TAC []) >> fs [] >>
+      Cases_on `enable_stg 3 (agp32 fext fbits t)` >-
+       (subgoal `I' (4,SUC t) = I' (3,t)` >-
+         (fs [is_sch_def,is_sch_memory_def,Abbr `s`] >>
+          `enable_stg 4 (agp32 fext fbits t)`
+            by fs [enable_stg_def,agp32_MEM_state_flag_eq_WB_state_flag] >>
+          Cases_on `isMemOp_hw_op (agp32 fext fbits t)` >>
+          fs [enable_stg_def] >>
+          METIS_TAC [MEM_stg_op_agp32_ID_EX_write_disable,enable_stg_def]) >> fs [] >>
+        `THE (I' (2,t)) = THE (I' (5,t)) + 1`
+          by METIS_TAC [EX_MEM_NONE_ID_instr_index_with_WB_instr_plus_1] >> fs []) >>
+      `I' (3,SUC t) = I' (3,t)` by METIS_TAC [is_sch_def,is_sch_disable_def] >>
+      `THE (I' (2,t)) = THE (I' (5,t)) + 1`
+        by METIS_TAC [EX_MEM_NONE_ID_instr_index_with_WB_instr_plus_1] >> fs []) >>
+    `~enable_stg 5 (agp32 fext fbits t)` by fs [enable_stg_def] >>
+    `I' (5,SUC t) = I' (5,t)` by METIS_TAC [is_sch_def,is_sch_disable_def] >> fs []) >-
    (** I (3,SUC t) and I (5,t) are not NONE **)
-   (`s.WB.WB_state_flag` by fs [Abbr `s`,enable_stg_def,agp32_ID_ID_write_enable_WB_state_flag] >>
-    `wb_data_vaild s` by fs [Abbr `s`,wb_data_vaild_def] >>
-    `(agp32 fext fbits (SUC t)).R = (FUNPOW Next (THE (I' (5,t))) a).R` by cheat >> fs [] >>
-    `(agp32 fext fbits (SUC t)).ID.ID_addrW = (30 >< 25) i`
-      by (fs [Abbr `i`,Abbr `s`,is_sch_def] >>
-          METIS_TAC [agp32_Rel_ag32_ID_addr_correct,addrW_def]) >> fs [] >>
-    subgoal `I' (2,SUC t) = I' (1,t)` >-
-     (fs [is_sch_def,is_sch_decode_def,Abbr `s`] >>
-      Cases_on `isJump_isa_op (I' (2,t)) a \/ isJump_isa_op (I' (3,t)) a` >>
-      METIS_TAC []) >> fs [] >>
-    subgoal `I' (5,SUC t) = I' (4,t)` >-
-     (fs [is_sch_def,is_sch_writeback_def,is_sch_disable_def,Abbr `s`] >>
-      Cases_on `enable_stg 5 (agp32 fext fbits t)` >>
-      METIS_TAC []) >> fs [] >>
-    subgoal `I' (4,SUC t) = I' (3,t)` >-
-     (fs [is_sch_def,is_sch_memory_def,Abbr `s`] >>
-      `enable_stg 4 (agp32 fext fbits t)`
-        by fs [enable_stg_def,agp32_ID_ID_write_enable_MEM_state_flag] >>
-      Cases_on `isMemOp_hw_op (agp32 fext fbits t)` >>
-      fs [enable_stg_def] >>
-      METIS_TAC [MEM_stg_op_agp32_ID_EX_write_disable,
-                 agp32_ID_ID_write_enable_and_ID_EX_write_enable]) >> fs [] >>
-    subgoal `I' (3,SUC t) = I' (2,t)` >-
-     (fs [is_sch_def,is_sch_execute_def,Abbr `s`] >>
-      `enable_stg 3 (agp32 fext fbits t)`
-        by fs [enable_stg_def,agp32_ID_ID_write_enable_and_ID_EX_write_enable] >>
-      Cases_on `isJump_isa_op (I' (3,t)) a` >-
-       METIS_TAC [isJump_isa_op_not_none] >>
-      Cases_on `~reg_data_hazard (agp32 fext fbits t)` >>
-      METIS_TAC []) >> fs [] >>
-    `THE (I' (2,t)) = THE (I' (5,t)) + 1`
-      by METIS_TAC [EX_MEM_NONE_ID_instr_index_with_WB_instr_plus_1] >>
-    `THE (I' (5,t)) = THE (I' (2,t)) - 1` by fs [] >>
-    `THE (I' (1,t)) = THE (I' (2,t)) + 1`
-      by METIS_TAC [IF_instr_index_with_ID_instr_plus_1] >> fs [] >>
-    METIS_TAC [reg_adr_update_isa_not_change_data]) >-
+   (Cases_on `s.WB.WB_state_flag` >-
+     (`wb_data_vaild s` by fs [Abbr `s`,wb_data_vaild_def] >>
+      `(agp32 fext fbits (SUC t)).R = (FUNPOW Next (THE (I' (5,t))) a).R` by cheat >> fs [] >>
+      `(agp32 fext fbits (SUC t)).ID.ID_addrW = (30 >< 25) i`
+        by (fs [Abbr `i`,Abbr `s`,is_sch_def] >>
+            METIS_TAC [agp32_Rel_ag32_ID_addr_correct,addrW_def]) >> fs [] >>
+       Cases_on `enable_stg 2 (agp32 fext fbits t)` >-
+       (subgoal `I' (2,SUC t) = I' (1,t)` >-
+         (fs [is_sch_def,is_sch_decode_def,Abbr `s`] >>
+          METIS_TAC []) >> fs [] >>
+        subgoal `I' (5,SUC t) = I' (4,t)` >-
+         (fs [is_sch_def,is_sch_writeback_def,is_sch_disable_def,Abbr `s`] >>
+          Cases_on `enable_stg 5 (agp32 fext fbits t)` >>
+          METIS_TAC []) >> fs [] >>
+        subgoal `I' (4,SUC t) = I' (3,t)` >-
+         (fs [is_sch_def,is_sch_memory_def,Abbr `s`] >>
+          `enable_stg 4 (agp32 fext fbits t)`
+            by fs [enable_stg_def,agp32_ID_ID_write_enable_MEM_state_flag] >>
+          Cases_on `isMemOp_hw_op (agp32 fext fbits t)` >>
+          fs [enable_stg_def] >>
+          METIS_TAC [MEM_stg_op_agp32_ID_EX_write_disable,
+                     agp32_ID_ID_write_enable_and_ID_EX_write_enable]) >> fs [] >>
+        subgoal `I' (3,SUC t) = I' (2,t)` >-
+         (fs [is_sch_def,is_sch_execute_def,Abbr `s`] >>
+          `enable_stg 3 (agp32 fext fbits t)`
+            by fs [enable_stg_def,agp32_ID_ID_write_enable_and_ID_EX_write_enable] >>
+          Cases_on `isJump_isa_op (I' (3,t)) a` >-
+           METIS_TAC [isJump_isa_op_not_none] >>
+          Cases_on `~reg_data_hazard (agp32 fext fbits t)` >>
+          METIS_TAC []) >> fs [] >>
+        `THE (I' (2,t)) = THE (I' (5,t)) + 1`
+          by METIS_TAC [EX_MEM_NONE_ID_instr_index_with_WB_instr_plus_1] >>
+        `THE (I' (5,t)) = THE (I' (2,t)) - 1` by fs [] >>
+        `THE (I' (1,t)) = THE (I' (2,t)) + 1`
+          by METIS_TAC [IF_instr_index_with_ID_instr_plus_1] >> fs [] >>
+        METIS_TAC [reg_adr_update_isa_not_change_data]) >>
+      `I' (2,SUC t) = I' (2,t)` by fs [is_sch_def,is_sch_disable_def] >>
+      subgoal `I' (5,SUC t) = I' (4,t)` >-
+       (fs [is_sch_def,is_sch_writeback_def,is_sch_disable_def,Abbr `s`] >>
+        Cases_on `enable_stg 5 (agp32 fext fbits t)` >>
+        METIS_TAC []) >> fs [] >>
+      Cases_on `enable_stg 3 (agp32 fext fbits t)` >-
+       (subgoal `I' (4,SUC t) = I' (3,t)` >-
+         (fs [is_sch_def,is_sch_memory_def,Abbr `s`] >>
+          `enable_stg 4 (agp32 fext fbits t)`
+            by fs [enable_stg_def,agp32_MEM_state_flag_eq_WB_state_flag] >>
+          Cases_on `isMemOp_hw_op (agp32 fext fbits t)` >>
+          fs [enable_stg_def] >>
+          METIS_TAC [MEM_stg_op_agp32_ID_EX_write_disable,enable_stg_def]) >> fs [] >>
+        `THE (I' (2,t)) = THE (I' (5,t)) + 1`
+          by METIS_TAC [EX_MEM_NONE_ID_instr_index_with_WB_instr_plus_1] >> fs []) >>
+      `I' (3,SUC t) = I' (3,t)` by METIS_TAC [is_sch_def,is_sch_disable_def] >> fs [] >>
+      `THE (I' (3,t)) = THE (I' (5,t)) + 1`
+        by METIS_TAC [EX_instr_index_with_WB_instr_plus_1_MEM_NONE] >>
+      `THE (I' (5,t)) = THE (I' (3,t)) - 1` by fs [] >>
+      `THE (I' (2,t)) = THE (I' (3,t)) + 1`
+        by METIS_TAC [ID_instr_index_with_EX_instr_plus_1] >> fs [] >>
+      METIS_TAC [reg_adr_update_isa_not_change_data]) >>
+    `~enable_stg 5 (agp32 fext fbits t)` by fs [enable_stg_def] >>
+    `I' (5,SUC t) = I' (5,t)` by METIS_TAC [is_sch_def,is_sch_disable_def] >> fs []) >-
    (** I (4,SUC t) and I (5,t) are not NONE **)
-   (`s.WB.WB_state_flag` by fs [Abbr `s`,enable_stg_def,agp32_ID_ID_write_enable_WB_state_flag] >>
-    `wb_data_vaild s` by fs [Abbr `s`,wb_data_vaild_def] >>
-    `(agp32 fext fbits (SUC t)).R = (FUNPOW Next (THE (I' (5,t))) a).R` by cheat >> fs [] >>
-    `(agp32 fext fbits (SUC t)).ID.ID_addrW = (30 >< 25) i`
-      by (fs [Abbr `i`,Abbr `s`,is_sch_def] >>
-          METIS_TAC [agp32_Rel_ag32_ID_addr_correct,addrW_def]) >> fs [] >>
-    subgoal `THE (I' (4,SUC t)) = THE (I' (5,t)) + 1` >-
-     (`I' (5,SUC t) = I' (4,t)`
+   (Cases_on`s.WB.WB_state_flag` >-
+     (`wb_data_vaild s` by fs [Abbr `s`,wb_data_vaild_def] >>
+      `(agp32 fext fbits (SUC t)).R = (FUNPOW Next (THE (I' (5,t))) a).R` by cheat >> fs [] >>
+      `(agp32 fext fbits (SUC t)).ID.ID_addrW = (30 >< 25) i`
+        by (fs [Abbr `i`,Abbr `s`,is_sch_def] >>
+            METIS_TAC [agp32_Rel_ag32_ID_addr_correct,addrW_def]) >> fs [] >>
+      Cases_on `enable_stg 2 (agp32 fext fbits t)` >-
+       (subgoal `THE (I' (4,SUC t)) = THE (I' (5,t)) + 1` >-
+         (`I' (5,SUC t) = I' (4,t)`
+            by (fs [is_sch_def,is_sch_writeback_def,is_sch_disable_def,Abbr `s`] >>
+                Cases_on `enable_stg 5 (agp32 fext fbits t)` >>
+                METIS_TAC []) >>
+          `I' (4,SUC t) = I' (3,t)`
+            by (fs [is_sch_def,is_sch_memory_def,Abbr `s`] >>
+                `enable_stg 4 (agp32 fext fbits t)`
+                  by fs [enable_stg_def,agp32_ID_ID_write_enable_MEM_state_flag] >>
+                Cases_on `isMemOp_hw_op (agp32 fext fbits t)` >>
+                fs [enable_stg_def] >>
+                METIS_TAC [MEM_stg_op_agp32_ID_EX_write_disable,
+                           agp32_ID_ID_write_enable_and_ID_EX_write_enable]) >> fs [] >>
+          METIS_TAC [EX_instr_index_with_WB_instr_plus_1_MEM_NONE]) >>
+        `THE (I' (5,t)) = THE (I' (4,SUC t)) - 1` by fs [] >> fs [] >>
+        `(FUNPOW Next (THE (I' (4,SUC t)) − 1) a).R ((30 >< 25) i) =
+        (FUNPOW Next (THE (I' (4,SUC t))) a).R ((30 >< 25) i)`
+          by METIS_TAC [reg_adr_update_isa_not_change_data] >> fs [] >>
+        `THE (I' (2,SUC t)) = THE (I' (4,SUC t)) + 1`
+          by METIS_TAC [EX_NONE_ID_instr_index_with_MEM_instr_plus_1] >> fs []) >>
+      `I' (2,SUC t) = I' (2,t)` by fs [is_sch_def,is_sch_disable_def] >>
+      subgoal `I' (4,SUC t) = I' (3,t)` >-
+       (fs [is_sch_def,is_sch_memory_def] >>
+        `enable_stg 4 (agp32 fext fbits t)`
+          by fs [enable_stg_def,agp32_MEM_state_flag_eq_WB_state_flag] >>
+        Cases_on `isMemOp_hw_op (agp32 fext fbits t)` >- METIS_TAC [] >> fs []) >>
+      `I' (5,SUC t) = I' (4,t)`
         by (fs [is_sch_def,is_sch_writeback_def,is_sch_disable_def,Abbr `s`] >>
             Cases_on `enable_stg 5 (agp32 fext fbits t)` >>
-            METIS_TAC []) >>
-      `I' (4,SUC t) = I' (3,t)`
-          by (fs [is_sch_def,is_sch_memory_def,Abbr `s`] >>
-              `enable_stg 4 (agp32 fext fbits t)`
-                by fs [enable_stg_def,agp32_ID_ID_write_enable_MEM_state_flag] >>
-              Cases_on `isMemOp_hw_op (agp32 fext fbits t)` >>
-              fs [enable_stg_def] >>
-              METIS_TAC [MEM_stg_op_agp32_ID_EX_write_disable,
-                         agp32_ID_ID_write_enable_and_ID_EX_write_enable]) >> fs [] >>
-      METIS_TAC [EX_instr_index_with_WB_instr_plus_1_MEM_NONE]) >>
-    `THE (I' (5,t)) = THE (I' (4,SUC t)) - 1` by fs [] >> fs [] >>
-    `(FUNPOW Next (THE (I' (4,SUC t)) − 1) a).R ((30 >< 25) i) =
-    (FUNPOW Next (THE (I' (4,SUC t))) a).R ((30 >< 25) i)`
-      by METIS_TAC [reg_adr_update_isa_not_change_data] >> fs [] >>
-    `THE (I' (2,SUC t)) = THE (I' (4,SUC t)) + 1`
-      by METIS_TAC [EX_NONE_ID_instr_index_with_MEM_instr_plus_1] >> fs []) >-
+            METIS_TAC []) >> fs [] >>
+      `THE (I' (3,t)) = THE (I' (5,t)) + 1`
+        by METIS_TAC [EX_instr_index_with_WB_instr_plus_1_MEM_NONE] >>
+      `THE (I' (5,t)) = THE (I' (3,t)) - 1` by fs [] >>
+      `THE (I' (2,t)) = THE (I' (3,t)) + 1`
+        by METIS_TAC [ID_instr_index_with_EX_instr_plus_1] >> fs [] >>
+      METIS_TAC [reg_adr_update_isa_not_change_data]) >>
+    `~enable_stg 5 (agp32 fext fbits t)` by fs [enable_stg_def] >>
+    `I' (5,SUC t) = I' (5,t)` by METIS_TAC [is_sch_def,is_sch_disable_def] >> fs []) >-
    (** I (3,SUC t), I (4,SUC t) and I (5,t) are not NONE **)
-   (`s.WB.WB_state_flag` by fs [Abbr `s`,enable_stg_def,agp32_ID_ID_write_enable_WB_state_flag] >>
-    `wb_data_vaild s` by fs [Abbr `s`,wb_data_vaild_def] >>
+   (Cases_on `s.WB.WB_state_flag` >-
+     (`wb_data_vaild s` by fs [Abbr `s`,wb_data_vaild_def] >>
+      `(agp32 fext fbits (SUC t)).R = (FUNPOW Next (THE (I' (5,t))) a).R` by cheat >> fs [] >>
+      `(agp32 fext fbits (SUC t)).ID.ID_addrW = (30 >< 25) i`
+        by (fs [Abbr `i`,Abbr `s`,is_sch_def] >>
+            METIS_TAC [agp32_Rel_ag32_ID_addr_correct,addrW_def]) >> fs [] >>
+      Cases_on `enable_stg 2 (agp32 fext fbits t)` >-
+       (subgoal `THE (I' (4,SUC t)) = THE (I' (5,t)) + 1` >-
+         (`I' (5,SUC t) = I' (4,t)`
+            by (fs [is_sch_def,is_sch_writeback_def,is_sch_disable_def,Abbr `s`] >>
+                Cases_on `enable_stg 5 (agp32 fext fbits t)` >>
+                METIS_TAC []) >>
+          `I' (4,SUC t) = I' (3,t)`
+            by (fs [is_sch_def,is_sch_memory_def,Abbr `s`] >>
+                `enable_stg 4 (agp32 fext fbits t)`
+                  by fs [enable_stg_def,agp32_ID_ID_write_enable_MEM_state_flag] >>
+                Cases_on `isMemOp_hw_op (agp32 fext fbits t)` >>
+                fs [enable_stg_def] >>
+                METIS_TAC [MEM_stg_op_agp32_ID_EX_write_disable,
+                           agp32_ID_ID_write_enable_and_ID_EX_write_enable]) >> fs [] >>
+          METIS_TAC [EX_instr_index_with_WB_instr_plus_1_MEM_NONE]) >>
+        `THE (I' (5,t)) = THE (I' (4,SUC t)) - 1` by fs [] >> fs [] >>
+        `(FUNPOW Next (THE (I' (4,SUC t)) − 1) a).R ((30 >< 25) i) =
+        (FUNPOW Next (THE (I' (4,SUC t))) a).R ((30 >< 25) i)`
+          by METIS_TAC [reg_adr_update_isa_not_change_data] >> fs [] >>
+        `THE (I' (3,SUC t)) = THE (I' (4,SUC t)) + 1`
+          by METIS_TAC [EX_instr_index_with_MEM_instr_plus_1] >>
+        `THE (I' (2,SUC t)) = THE (I' (3,SUC t)) + 1`
+          by METIS_TAC [ID_instr_index_with_EX_instr_plus_1] >> fs [] >>
+        `THE (I' (4,SUC t)) = THE (I' (3,SUC t)) - 1` by FULL_SIMP_TAC std_ss [] >>
+        METIS_TAC [reg_adr_update_isa_not_change_data]) >>
+      `I' (2,SUC t) = I' (2,t)` by fs [is_sch_def,is_sch_disable_def] >>
+      subgoal `I' (4,SUC t) = I' (3,t)` >-
+       (fs [is_sch_def,is_sch_memory_def] >>
+        `enable_stg 4 (agp32 fext fbits t)`
+          by fs [enable_stg_def,agp32_MEM_state_flag_eq_WB_state_flag] >>
+        Cases_on `isMemOp_hw_op (agp32 fext fbits t)` >- METIS_TAC [] >> fs []) >>
+      `I' (5,SUC t) = I' (4,t)`
+        by (fs [is_sch_def,is_sch_writeback_def,is_sch_disable_def,Abbr `s`] >>
+            Cases_on `enable_stg 5 (agp32 fext fbits t)` >>
+            METIS_TAC []) >> fs [] >>
+      `THE (I' (3,t)) = THE (I' (5,t)) + 1`
+        by METIS_TAC [EX_instr_index_with_WB_instr_plus_1_MEM_NONE] >>
+      `THE (I' (5,t)) = THE (I' (3,t)) - 1` by fs [] >>
+      `THE (I' (2,t)) = THE (I' (3,t)) + 1`
+        by METIS_TAC [ID_instr_index_with_EX_instr_plus_1] >> fs [] >>
+      METIS_TAC [reg_adr_update_isa_not_change_data]) >>
+    `~enable_stg 5 (agp32 fext fbits t)` by fs [enable_stg_def] >>
+    `I' (5,SUC t) = I' (5,t)` by METIS_TAC [is_sch_def,is_sch_disable_def] >> fs []) >-
+   (** I (5,SUC t) and I (5,t) are not NONE **)
+   (Cases_on `s.WB.WB_state_flag` >-
+     (`wb_data_vaild s` by fs [Abbr `s`,wb_data_vaild_def] >>
+      `(agp32 fext fbits (SUC t)).R = (FUNPOW Next (THE (I' (5,t))) a).R` by cheat >> fs [] >>
+      `(agp32 fext fbits (SUC t)).ID.ID_addrW = (30 >< 25) i`
+        by (fs [Abbr `i`,Abbr `s`,is_sch_def] >>
+            METIS_TAC [agp32_Rel_ag32_ID_addr_correct,addrW_def]) >> fs [] >>
+      `enable_stg 5 (agp32 fext fbits t)`
+        by fs [enable_stg_def,agp32_ID_ID_write_enable_WB_state_flag] >>
+      `THE (I' (5,SUC t)) = THE (I' (5,t)) + 1` by METIS_TAC [WB_instr_index_t_SUC_t_enable] >>
+      `THE (I' (5,t)) = THE (I' (5,SUC t)) - 1` by fs [] >> fs [] >>
+      `(FUNPOW Next (THE (I' (5,SUC t)) − 1) a).R ((30 >< 25) i) =
+      (FUNPOW Next (THE (I' (5,SUC t))) a).R ((30 >< 25) i)`
+        by METIS_TAC [reg_adr_update_isa_not_change_data] >> fs [] >>
+      `THE (I' (2,SUC t)) = THE (I' (5,SUC t)) + 1`
+        by METIS_TAC [EX_MEM_NONE_ID_instr_index_with_WB_instr_plus_1] >> fs []) >>
+    `~enable_stg 5 (agp32 fext fbits t)` by fs [enable_stg_def] >>
+    `~enable_stg 4 (agp32 fext fbits t)`
+      by fs [enable_stg_def,agp32_MEM_state_flag_eq_WB_state_flag] >>
+    `~(agp32 fext fbits t).ID.ID_ID_write_enable /\ ~(agp32 fext fbits t).ID.ID_EX_write_enable`
+      by METIS_TAC [agp32_ID_EX_write_enable_WB_state_flag,agp32_ID_ID_write_enable_WB_state_flag] >>
+    `~enable_stg 2 (agp32 fext fbits t) /\
+    ~enable_stg 3 (agp32 fext fbits t)` by fs [enable_stg_def] >>
+    `(agp32 fext fbits (SUC t)).ID.ID_addrW = s.ID.ID_addrW`
+      by METIS_TAC [Abbr `s`,is_sch_def,agp32_ID_disabled_ID_addr_unchanged] >>
+    `(agp32 fext fbits (SUC t)).ID.ID_addrW_disable = (agp32 fext fbits t).ID.ID_addrW_disable`
+      by METIS_TAC [Abbr `s`,is_sch_def,agp32_ID_disabled_ID_flag_unchanged] >>
+    `(agp32 fext fbits (SUC t)).ID.ID_read_dataW = (agp32 fext fbits t).ID.ID_read_dataW`
+      by METIS_TAC [Abbr `s`,is_sch_def,agp32_ID_disabled_ID_read_data_unchanged] >>
+    `(I' (2,SUC t) = I' (2,t)) /\ (I' (3,SUC t) = I' (3,t)) /\
+    (I' (4,SUC t) = I' (4,t)) /\ (I' (5,SUC t) = I' (5,t))` by METIS_TAC [is_sch_def,is_sch_disable_def] >>
+    fs [Rel_def,ID_reg_data_Rel_def,reg_dataW_def,addrW_def] >> METIS_TAC []) >-
+   (** I (3,SUC t), I (5,SUC t) and I (5,t) are not NONE **)
+   (Cases_on `s.WB.WB_state_flag` >-
+     (`wb_data_vaild s` by fs [Abbr `s`,wb_data_vaild_def] >>
+      `(agp32 fext fbits (SUC t)).R = (FUNPOW Next (THE (I' (5,t))) a).R` by cheat >> fs [] >>
+      `(agp32 fext fbits (SUC t)).ID.ID_addrW = (30 >< 25) i`
+        by (fs [Abbr `i`,Abbr `s`,is_sch_def] >>
+            METIS_TAC [agp32_Rel_ag32_ID_addr_correct,addrW_def]) >> fs [] >>
+      `enable_stg 5 (agp32 fext fbits t)`
+        by fs [enable_stg_def,agp32_ID_ID_write_enable_WB_state_flag] >>
+      `THE (I' (5,SUC t)) = THE (I' (5,t)) + 1` by METIS_TAC [WB_instr_index_t_SUC_t_enable] >>
+      `THE (I' (5,t)) = THE (I' (5,SUC t)) - 1` by fs [] >> fs [] >>
+      `(FUNPOW Next (THE (I' (5,SUC t)) − 1) a).R ((30 >< 25) i) =
+      (FUNPOW Next (THE (I' (5,SUC t))) a).R ((30 >< 25) i)`
+        by METIS_TAC [reg_adr_update_isa_not_change_data] >> fs [] >>
+      `THE (I' (3,SUC t)) = THE (I' (5,SUC t)) + 1`
+        by METIS_TAC [EX_instr_index_with_WB_instr_plus_1_MEM_NONE] >>
+      `THE (I' (2,SUC t)) = THE (I' (3,SUC t)) + 1`
+        by METIS_TAC [ID_instr_index_with_EX_instr_plus_1] >> fs [] >>
+      `THE (I' (5,SUC t)) = THE (I' (3,SUC t)) - 1` by fs [] >>
+      METIS_TAC [reg_adr_update_isa_not_change_data]) >>
+    `~enable_stg 5 (agp32 fext fbits t)` by fs [enable_stg_def] >>
+    `~enable_stg 4 (agp32 fext fbits t)`
+      by fs [enable_stg_def,agp32_MEM_state_flag_eq_WB_state_flag] >>
+    `~(agp32 fext fbits t).ID.ID_ID_write_enable /\ ~(agp32 fext fbits t).ID.ID_EX_write_enable`
+      by METIS_TAC [agp32_ID_EX_write_enable_WB_state_flag,agp32_ID_ID_write_enable_WB_state_flag] >>
+    `~enable_stg 2 (agp32 fext fbits t) /\
+    ~enable_stg 3 (agp32 fext fbits t)` by fs [enable_stg_def] >>
+    `(agp32 fext fbits (SUC t)).ID.ID_addrW = s.ID.ID_addrW`
+      by METIS_TAC [Abbr `s`,is_sch_def,agp32_ID_disabled_ID_addr_unchanged] >>
+    `(agp32 fext fbits (SUC t)).ID.ID_addrW_disable = (agp32 fext fbits t).ID.ID_addrW_disable`
+      by METIS_TAC [Abbr `s`,is_sch_def,agp32_ID_disabled_ID_flag_unchanged] >>
+    `(agp32 fext fbits (SUC t)).ID.ID_read_dataW = (agp32 fext fbits t).ID.ID_read_dataW`
+      by METIS_TAC [Abbr `s`,is_sch_def,agp32_ID_disabled_ID_read_data_unchanged] >>
+    `(I' (2,SUC t) = I' (2,t)) /\ (I' (3,SUC t) = I' (3,t)) /\
+    (I' (4,SUC t) = I' (4,t)) /\ (I' (5,SUC t) = I' (5,t))` by METIS_TAC [is_sch_def,is_sch_disable_def] >>
+    fs [Rel_def,ID_reg_data_Rel_def,reg_dataW_def,addrW_def] >> METIS_TAC []) >-
+   (** I (4,SUC t), I (5,SUC t) and I (5,t) are not NONE **)
+   (Cases_on `s.WB.WB_state_flag` >-
+     (`wb_data_vaild s` by fs [Abbr `s`,wb_data_vaild_def] >>
+      `(agp32 fext fbits (SUC t)).R = (FUNPOW Next (THE (I' (5,t))) a).R` by cheat >> fs [] >>
+      `(agp32 fext fbits (SUC t)).ID.ID_addrW = (30 >< 25) i`
+        by (fs [Abbr `i`,Abbr `s`,is_sch_def] >>
+            METIS_TAC [agp32_Rel_ag32_ID_addr_correct,addrW_def]) >> fs [] >>
+      `enable_stg 5 (agp32 fext fbits t)`
+        by fs [enable_stg_def,agp32_ID_ID_write_enable_WB_state_flag] >>
+      `THE (I' (5,SUC t)) = THE (I' (5,t)) + 1` by METIS_TAC [WB_instr_index_t_SUC_t_enable] >>
+      `THE (I' (5,t)) = THE (I' (5,SUC t)) - 1` by fs [] >> fs [] >>
+      `(FUNPOW Next (THE (I' (5,SUC t)) − 1) a).R ((30 >< 25) i) =
+      (FUNPOW Next (THE (I' (5,SUC t))) a).R ((30 >< 25) i)`
+        by METIS_TAC [reg_adr_update_isa_not_change_data] >> fs [] >>
+      `THE (I' (4,SUC t)) = THE (I' (5,SUC t)) + 1`
+        by METIS_TAC [MEM_instr_index_with_WB_instr_plus_1] >>
+      `THE (I' (2,SUC t)) = THE (I' (4,SUC t)) + 1`
+        by METIS_TAC [EX_NONE_ID_instr_index_with_MEM_instr_plus_1] >> fs [] >>
+      `THE (I' (5,SUC t)) = THE (I' (4,SUC t)) - 1` by fs [] >>
+      METIS_TAC [reg_adr_update_isa_not_change_data]) >>
+    `~enable_stg 5 (agp32 fext fbits t)` by fs [enable_stg_def] >>
+    `~enable_stg 4 (agp32 fext fbits t)`
+      by fs [enable_stg_def,agp32_MEM_state_flag_eq_WB_state_flag] >>
+    `~(agp32 fext fbits t).ID.ID_ID_write_enable /\ ~(agp32 fext fbits t).ID.ID_EX_write_enable`
+      by METIS_TAC [agp32_ID_EX_write_enable_WB_state_flag,agp32_ID_ID_write_enable_WB_state_flag] >>
+    `~enable_stg 2 (agp32 fext fbits t) /\
+    ~enable_stg 3 (agp32 fext fbits t)` by fs [enable_stg_def] >>
+    `(agp32 fext fbits (SUC t)).ID.ID_addrW = s.ID.ID_addrW`
+      by METIS_TAC [Abbr `s`,is_sch_def,agp32_ID_disabled_ID_addr_unchanged] >>
+    `(agp32 fext fbits (SUC t)).ID.ID_addrW_disable = (agp32 fext fbits t).ID.ID_addrW_disable`
+      by METIS_TAC [Abbr `s`,is_sch_def,agp32_ID_disabled_ID_flag_unchanged] >>
+    `(agp32 fext fbits (SUC t)).ID.ID_read_dataW = (agp32 fext fbits t).ID.ID_read_dataW`
+      by METIS_TAC [Abbr `s`,is_sch_def,agp32_ID_disabled_ID_read_data_unchanged] >>
+    `(I' (2,SUC t) = I' (2,t)) /\ (I' (3,SUC t) = I' (3,t)) /\
+    (I' (4,SUC t) = I' (4,t)) /\ (I' (5,SUC t) = I' (5,t))` by METIS_TAC [is_sch_def,is_sch_disable_def] >>
+    fs [Rel_def,ID_reg_data_Rel_def,reg_dataW_def,addrW_def] >> METIS_TAC []) >>
+  (** all are not NONE **)
+  Cases_on `s.WB.WB_state_flag` >-
+   (`wb_data_vaild s` by fs [Abbr `s`,wb_data_vaild_def] >>
     `(agp32 fext fbits (SUC t)).R = (FUNPOW Next (THE (I' (5,t))) a).R` by cheat >> fs [] >>
     `(agp32 fext fbits (SUC t)).ID.ID_addrW = (30 >< 25) i`
       by (fs [Abbr `i`,Abbr `s`,is_sch_def] >>
           METIS_TAC [agp32_Rel_ag32_ID_addr_correct,addrW_def]) >> fs [] >>
-    subgoal `THE (I' (4,SUC t)) = THE (I' (5,t)) + 1` >-
-     (`I' (5,SUC t) = I' (4,t)`
-        by (fs [is_sch_def,is_sch_writeback_def,is_sch_disable_def,Abbr `s`] >>
-            Cases_on `enable_stg 5 (agp32 fext fbits t)` >>
-            METIS_TAC []) >>
-      `I' (4,SUC t) = I' (3,t)`
-          by (fs [is_sch_def,is_sch_memory_def,Abbr `s`] >>
-              `enable_stg 4 (agp32 fext fbits t)`
-                by fs [enable_stg_def,agp32_ID_ID_write_enable_MEM_state_flag] >>
-              Cases_on `isMemOp_hw_op (agp32 fext fbits t)` >>
-              fs [enable_stg_def] >>
-              METIS_TAC [MEM_stg_op_agp32_ID_EX_write_disable,
-                         agp32_ID_ID_write_enable_and_ID_EX_write_enable]) >> fs [] >>
-      METIS_TAC [EX_instr_index_with_WB_instr_plus_1_MEM_NONE]) >>
-    `THE (I' (5,t)) = THE (I' (4,SUC t)) - 1` by fs [] >> fs [] >>
+    `enable_stg 5 (agp32 fext fbits t)`
+      by fs [enable_stg_def,agp32_ID_ID_write_enable_WB_state_flag] >>
+    `THE (I' (5,SUC t)) = THE (I' (5,t)) + 1` by METIS_TAC [WB_instr_index_t_SUC_t_enable] >>
+    `THE (I' (5,t)) = THE (I' (5,SUC t)) - 1` by fs [] >> fs [] >>
+    `(FUNPOW Next (THE (I' (5,SUC t)) − 1) a).R ((30 >< 25) i) =
+    (FUNPOW Next (THE (I' (5,SUC t))) a).R ((30 >< 25) i)`
+      by METIS_TAC [reg_adr_update_isa_not_change_data] >> fs [] >>
+    qpat_x_assum `THE (I' (5,SUC t)) = _` (fn thm => all_tac)  >>
+    `THE (I' (4,SUC t)) = THE (I' (5,SUC t)) + 1`
+      by METIS_TAC [MEM_instr_index_with_WB_instr_plus_1] >>
+    `THE (I' (5,SUC t)) = THE (I' (4,SUC t)) - 1` by fs [] >> fs [] >>
     `(FUNPOW Next (THE (I' (4,SUC t)) − 1) a).R ((30 >< 25) i) =
     (FUNPOW Next (THE (I' (4,SUC t))) a).R ((30 >< 25) i)`
       by METIS_TAC [reg_adr_update_isa_not_change_data] >> fs [] >>
@@ -1625,90 +2195,23 @@ Proof
     `THE (I' (2,SUC t)) = THE (I' (3,SUC t)) + 1`
       by METIS_TAC [ID_instr_index_with_EX_instr_plus_1] >> fs [] >>
     `THE (I' (4,SUC t)) = THE (I' (3,SUC t)) - 1` by FULL_SIMP_TAC std_ss [] >>
-    METIS_TAC [reg_adr_update_isa_not_change_data]) >-
-   (** I (5,SUC t) and I (5,t) are not NONE **)
-   (`s.WB.WB_state_flag` by fs [Abbr `s`,enable_stg_def,agp32_ID_ID_write_enable_WB_state_flag] >>
-    `wb_data_vaild s` by fs [Abbr `s`,wb_data_vaild_def] >>
-    `(agp32 fext fbits (SUC t)).R = (FUNPOW Next (THE (I' (5,t))) a).R` by cheat >> fs [] >>
-    `(agp32 fext fbits (SUC t)).ID.ID_addrW = (30 >< 25) i`
-      by (fs [Abbr `i`,Abbr `s`,is_sch_def] >>
-          METIS_TAC [agp32_Rel_ag32_ID_addr_correct,addrW_def]) >> fs [] >>
-    `enable_stg 5 (agp32 fext fbits t)`
-      by fs [enable_stg_def,agp32_ID_ID_write_enable_WB_state_flag] >>
-    `THE (I' (5,SUC t)) = THE (I' (5,t)) + 1` by METIS_TAC [WB_instr_index_t_SUC_t_enable] >>
-    `THE (I' (5,t)) = THE (I' (5,SUC t)) - 1` by fs [] >> fs [] >>
-    `(FUNPOW Next (THE (I' (5,SUC t)) − 1) a).R ((30 >< 25) i) =
-    (FUNPOW Next (THE (I' (5,SUC t))) a).R ((30 >< 25) i)`
-      by METIS_TAC [reg_adr_update_isa_not_change_data] >> fs [] >>
-    `THE (I' (2,SUC t)) = THE (I' (5,SUC t)) + 1`
-      by METIS_TAC [EX_MEM_NONE_ID_instr_index_with_WB_instr_plus_1] >> fs []) >-
-   (** I (3,SUC t), I (5,SUC t) and I (5,t) are not NONE **)
-   (`s.WB.WB_state_flag` by fs [Abbr `s`,enable_stg_def,agp32_ID_ID_write_enable_WB_state_flag] >>
-    `wb_data_vaild s` by fs [Abbr `s`,wb_data_vaild_def] >>
-    `(agp32 fext fbits (SUC t)).R = (FUNPOW Next (THE (I' (5,t))) a).R` by cheat >> fs [] >>
-    `(agp32 fext fbits (SUC t)).ID.ID_addrW = (30 >< 25) i`
-      by (fs [Abbr `i`,Abbr `s`,is_sch_def] >>
-          METIS_TAC [agp32_Rel_ag32_ID_addr_correct,addrW_def]) >> fs [] >>
-    `enable_stg 5 (agp32 fext fbits t)`
-      by fs [enable_stg_def,agp32_ID_ID_write_enable_WB_state_flag] >>
-    `THE (I' (5,SUC t)) = THE (I' (5,t)) + 1` by METIS_TAC [WB_instr_index_t_SUC_t_enable] >>
-    `THE (I' (5,t)) = THE (I' (5,SUC t)) - 1` by fs [] >> fs [] >>
-    `(FUNPOW Next (THE (I' (5,SUC t)) − 1) a).R ((30 >< 25) i) =
-    (FUNPOW Next (THE (I' (5,SUC t))) a).R ((30 >< 25) i)`
-      by METIS_TAC [reg_adr_update_isa_not_change_data] >> fs [] >>
-    `THE (I' (3,SUC t)) = THE (I' (5,SUC t)) + 1`
-      by METIS_TAC [EX_instr_index_with_WB_instr_plus_1_MEM_NONE] >>
-    `THE (I' (2,SUC t)) = THE (I' (3,SUC t)) + 1`
-      by METIS_TAC [ID_instr_index_with_EX_instr_plus_1] >> fs [] >>
-    `THE (I' (5,SUC t)) = THE (I' (3,SUC t)) - 1` by fs [] >>
-    METIS_TAC [reg_adr_update_isa_not_change_data]) >-
-   (** I (4,SUC t), I (5,SUC t) and I (5,t) are not NONE **)
-   (`s.WB.WB_state_flag` by fs [Abbr `s`,enable_stg_def,agp32_ID_ID_write_enable_WB_state_flag] >>
-    `wb_data_vaild s` by fs [Abbr `s`,wb_data_vaild_def] >>
-    `(agp32 fext fbits (SUC t)).R = (FUNPOW Next (THE (I' (5,t))) a).R` by cheat >> fs [] >>
-    `(agp32 fext fbits (SUC t)).ID.ID_addrW = (30 >< 25) i`
-      by (fs [Abbr `i`,Abbr `s`,is_sch_def] >>
-          METIS_TAC [agp32_Rel_ag32_ID_addr_correct,addrW_def]) >> fs [] >>
-    `enable_stg 5 (agp32 fext fbits t)`
-      by fs [enable_stg_def,agp32_ID_ID_write_enable_WB_state_flag] >>
-    `THE (I' (5,SUC t)) = THE (I' (5,t)) + 1` by METIS_TAC [WB_instr_index_t_SUC_t_enable] >>
-    `THE (I' (5,t)) = THE (I' (5,SUC t)) - 1` by fs [] >> fs [] >>
-    `(FUNPOW Next (THE (I' (5,SUC t)) − 1) a).R ((30 >< 25) i) =
-    (FUNPOW Next (THE (I' (5,SUC t))) a).R ((30 >< 25) i)`
-      by METIS_TAC [reg_adr_update_isa_not_change_data] >> fs [] >>
-    `THE (I' (4,SUC t)) = THE (I' (5,SUC t)) + 1`
-      by METIS_TAC [MEM_instr_index_with_WB_instr_plus_1] >>
-    `THE (I' (2,SUC t)) = THE (I' (4,SUC t)) + 1`
-      by METIS_TAC [EX_NONE_ID_instr_index_with_MEM_instr_plus_1] >> fs [] >>
-    `THE (I' (5,SUC t)) = THE (I' (4,SUC t)) - 1` by fs [] >>
     METIS_TAC [reg_adr_update_isa_not_change_data]) >>
-  (** all are not NONE **)
-  `s.WB.WB_state_flag` by fs [Abbr `s`,enable_stg_def,agp32_ID_ID_write_enable_WB_state_flag] >>
-  `wb_data_vaild s` by fs [Abbr `s`,wb_data_vaild_def] >>
-  `(agp32 fext fbits (SUC t)).R = (FUNPOW Next (THE (I' (5,t))) a).R` by cheat >> fs [] >>
-  `(agp32 fext fbits (SUC t)).ID.ID_addrW = (30 >< 25) i`
-    by (fs [Abbr `i`,Abbr `s`,is_sch_def] >>
-        METIS_TAC [agp32_Rel_ag32_ID_addr_correct,addrW_def]) >> fs [] >>
-  `enable_stg 5 (agp32 fext fbits t)`
-    by fs [enable_stg_def,agp32_ID_ID_write_enable_WB_state_flag] >>
-  `THE (I' (5,SUC t)) = THE (I' (5,t)) + 1` by METIS_TAC [WB_instr_index_t_SUC_t_enable] >>
-  `THE (I' (5,t)) = THE (I' (5,SUC t)) - 1` by fs [] >> fs [] >>
-  `(FUNPOW Next (THE (I' (5,SUC t)) − 1) a).R ((30 >< 25) i) =
-  (FUNPOW Next (THE (I' (5,SUC t))) a).R ((30 >< 25) i)`
-    by METIS_TAC [reg_adr_update_isa_not_change_data] >> fs [] >>
-  qpat_x_assum `THE (I' (5,SUC t)) = _` (fn thm => all_tac)  >>
-  `THE (I' (4,SUC t)) = THE (I' (5,SUC t)) + 1`
-    by METIS_TAC [MEM_instr_index_with_WB_instr_plus_1] >>
-  `THE (I' (5,SUC t)) = THE (I' (4,SUC t)) - 1` by fs [] >> fs [] >>
-  `(FUNPOW Next (THE (I' (4,SUC t)) − 1) a).R ((30 >< 25) i) =
-  (FUNPOW Next (THE (I' (4,SUC t))) a).R ((30 >< 25) i)`
-    by METIS_TAC [reg_adr_update_isa_not_change_data] >> fs [] >>
-  `THE (I' (3,SUC t)) = THE (I' (4,SUC t)) + 1`
-    by METIS_TAC [EX_instr_index_with_MEM_instr_plus_1] >>
-  `THE (I' (2,SUC t)) = THE (I' (3,SUC t)) + 1`
-    by METIS_TAC [ID_instr_index_with_EX_instr_plus_1] >> fs [] >>
-  `THE (I' (4,SUC t)) = THE (I' (3,SUC t)) - 1` by FULL_SIMP_TAC std_ss [] >>
-  METIS_TAC [reg_adr_update_isa_not_change_data]
+  `~enable_stg 5 (agp32 fext fbits t)` by fs [enable_stg_def] >>
+  `~enable_stg 4 (agp32 fext fbits t)`
+    by fs [enable_stg_def,agp32_MEM_state_flag_eq_WB_state_flag] >>
+  `~(agp32 fext fbits t).ID.ID_ID_write_enable /\ ~(agp32 fext fbits t).ID.ID_EX_write_enable`
+    by METIS_TAC [agp32_ID_EX_write_enable_WB_state_flag,agp32_ID_ID_write_enable_WB_state_flag] >>
+  `~enable_stg 2 (agp32 fext fbits t) /\
+  ~enable_stg 3 (agp32 fext fbits t)` by fs [enable_stg_def] >>
+  `(agp32 fext fbits (SUC t)).ID.ID_addrW = s.ID.ID_addrW`
+    by METIS_TAC [Abbr `s`,is_sch_def,agp32_ID_disabled_ID_addr_unchanged] >>
+  `(agp32 fext fbits (SUC t)).ID.ID_addrW_disable = (agp32 fext fbits t).ID.ID_addrW_disable`
+    by METIS_TAC [Abbr `s`,is_sch_def,agp32_ID_disabled_ID_flag_unchanged] >>
+  `(agp32 fext fbits (SUC t)).ID.ID_read_dataW = (agp32 fext fbits t).ID.ID_read_dataW`
+    by METIS_TAC [Abbr `s`,is_sch_def,agp32_ID_disabled_ID_read_data_unchanged] >>
+  `(I' (2,SUC t) = I' (2,t)) /\ (I' (3,SUC t) = I' (3,t)) /\
+  (I' (4,SUC t) = I' (4,t)) /\ (I' (5,SUC t) = I' (5,t))` by METIS_TAC [is_sch_def,is_sch_disable_def] >>
+  fs [Rel_def,ID_reg_data_Rel_def,reg_dataW_def,addrW_def] >> METIS_TAC []
 QED
 
 
@@ -1717,7 +2220,6 @@ Theorem agp32_Rel_ag32_ID_dataA_no_write_before:
   !fext fbits a t I.
     is_sch I (agp32 fext fbits) a ==>
     Rel I (fext t) (agp32 fext fbits (t-1)) (agp32 fext fbits t) a t ==>
-    enable_stg 2 (agp32 fext fbits t) ==>
     I (2,SUC t) <> NONE ==>
     ~(agp32 fext fbits (SUC t)).ID.ID_addrA_disable ==>
     ~reg_adr_update_isa (I (3,SUC t)) a (agp32 fext fbits (SUC t)).ID.ID_addrA ==>
@@ -1737,7 +2239,6 @@ Theorem agp32_Rel_ag32_ID_dataB_no_write_before:
   !fext fbits a t I.
     is_sch I (agp32 fext fbits) a ==>
     Rel I (fext t) (agp32 fext fbits (t-1)) (agp32 fext fbits t) a t ==>
-    enable_stg 2 (agp32 fext fbits t) ==>
     I (2,SUC t) <> NONE ==>
     ~(agp32 fext fbits (SUC t)).ID.ID_addrB_disable ==>
     ~reg_adr_update_isa (I (3,SUC t)) a (agp32 fext fbits (SUC t)).ID.ID_addrB ==>
@@ -1758,7 +2259,6 @@ Theorem agp32_Rel_ag32_ID_dataW_no_write_before:
   !fext fbits a t I.
     is_sch I (agp32 fext fbits) a ==>
     Rel I (fext t) (agp32 fext fbits (t-1)) (agp32 fext fbits t) a t ==>
-    enable_stg 2 (agp32 fext fbits t) ==>
     I (2,SUC t) <> NONE ==>
     ~(agp32 fext fbits (SUC t)).ID.ID_addrW_disable ==>
     ~reg_adr_update_isa (I (3,SUC t)) a (agp32 fext fbits (SUC t)).ID.ID_addrW ==>
@@ -1779,7 +2279,6 @@ Theorem agp32_Rel_ag32_ID_reg_data_Rel_correct:
   !fext fbits a t I.
     is_sch I (agp32 fext fbits) a ==>
     Rel I (fext t) (agp32 fext fbits (t-1)) (agp32 fext fbits t) a t ==>
-    enable_stg 2 (agp32 fext fbits t) ==>
     I (2,SUC t) <> NONE ==>
     ID_reg_data_Rel (agp32 fext fbits (SUC t)) a
                     (THE (I (2,SUC t))) (I (3,SUC t)) (I (4,SUC t)) (I (5,SUC t))
